MappingFunStatelessCircus.lhs
@@ -18,7 +18,7 @@ module MappingFunStatelessCircus
 where
 import AST
 import DefSets
-import Data.List
+import Data.List hiding (union, intersect)
 import FormatterToCSP
 import CRL
 
@@ -28,9 +28,9 @@ showexpr = zexpr_string (pinfo_extz 80)
 \begin{code}
 def_delta_mapping :: [(ZName, ZVar, ZExpr)] -> [ZExpr]
 def_delta_mapping [(n,(v,[]),t)] 
-  = [ZCall (ZVar ("\\mapsto",[])) (ZTuple [ZVar ((join_name n v),[]),t])]
+  = [ZCall (ZVar ("\\mapsto",[])) (ZTuple [ZVar ((join_name (join_name "st_var" n) v),[]),t])]
 def_delta_mapping ((n,(v,[]),t):xs) 
-  = [ZCall (ZVar ("\\mapsto",[])) (ZTuple [ZVar ((join_name n v),[]),t])] 
+  = [ZCall (ZVar ("\\mapsto",[])) (ZTuple [ZVar ((join_name (join_name "st_var" n) v),[]),t])] 
     ++ (def_delta_mapping xs)
 def_delta_mapping [] = []
 \end{code}
@@ -38,11 +38,12 @@ def_delta_mapping [] = []
 \begin{code}
 def_delta_name :: [(ZName, ZVar, ZExpr)] -> [ZBranch]
 def_delta_name [(n,(v,[]),t)] 
-  = [ZBranch0 ((join_name n v),[])]
+  = [ZBranch0 ((join_name (join_name "st_var" n) v),[])]
 def_delta_name ((n,(v,[]),t):xs) 
-  = [ZBranch0 ((join_name n v),[])] 
+  = [ZBranch0 ((join_name (join_name "st_var" n) v),[])] 
     ++ (def_delta_name xs)
 def_delta_name [] = []
+
 \end{code}
 \begin{code}
 get_pre_Circ_proc :: [ZPara] -> [ZPara]
@@ -55,7 +56,7 @@ get_pre_Circ_proc []
 \end{code}
 \begin{code}
 omega_Circus :: [ZPara] -> [ZPara]
-omega_Circus spec1
+omega_Circus spec
   = [ZGivenSetDecl ("UNIVERSE",[]),
       ZFreeTypeDef ("NAME",[]) (def_delta_name (def_mem_st_Circus_aux spec1)),
       ZAbbreviation ("BINDINGS",[]) (ZCall (ZVar ("\\fun",[])) (ZTuple [ZVar ("NAME",[]),ZVar ("UNIVERSE",[])])), 
@@ -63,11 +64,9 @@ omega_Circus spec1
       CircChannel [CChanDecl "mget" (ZCross [ZVar ("NAME",[]),ZVar ("UNIVERSE",[])]), CChanDecl "mset" (ZCross [ZVar ("NAME",[]),ZVar ("UNIVERSE",[])])],
       CircChannel [CChan "terminate"],
       CircChanSet "MEMi" (CChanSet ["mset","mget","terminate"])]
-    ++ (omega_Circus_aux spec spec)
+    ++ (omega_Circus_aux spec1 spec1)
     where 
-      spec = (map (rename_vars_ZPara1 (def_mem_st_Circus_aux spec1)) spec1)
-    -- HERE YOU HAVE TO PUT A AUXILIARY FUNCTION 
-    -- THAT WILL CHANGE THE NAE TO PROC_VAR
+      spec1 = (map (rename_vars_ZPara1 (def_mem_st_Circus_aux spec)) spec) -- renaming variables for highlighting which is state var from which process
 \end{code}
 \subsection{Creating the Memory process}
 \begin{code}
@@ -130,14 +129,14 @@ get_state_var_aux _ _ = []
 omega_Circus_aux :: [ZPara] -> [ZPara] -> [ZPara]
 
 omega_Circus_aux spec [(Process cp)]
-  = [(Process (omega_ProcDecl spec ncp))]
-  where
-    ncp = (rename_vars_ProcDecl1 (def_mem_st_Circus_aux spec) cp)
+  = [(Process (omega_ProcDecl spec cp))]
+  -- where
+  --   ncp = (rename_vars_ProcDecl1 (def_mem_st_Circus_aux spec) cp)
 omega_Circus_aux spec [x] = [x]
 omega_Circus_aux spec ((Process cp):xs)
-  = [(Process (omega_ProcDecl spec ncp))]++(omega_Circus_aux spec xs)
-  where
-    ncp = (rename_vars_ProcDecl1 (def_mem_st_Circus_aux spec) cp)
+  = [(Process (omega_ProcDecl spec cp))]++(omega_Circus_aux spec xs)
+  -- where
+  -- ncp = (rename_vars_ProcDecl1 (def_mem_st_Circus_aux spec) cp)
 omega_Circus_aux spec (x:xs)
   = [x]++(omega_Circus_aux spec xs)
 \end{code}
@@ -150,12 +149,12 @@ omega_Circus_aux spec (x:xs)
 omega_ProcDecl :: [ZPara] -> ProcDecl -> ProcDecl
 omega_ProcDecl spec (CGenProcess zn (x:xs) pd)
   = (CGenProcess zn (x:xs) (omega_ProcessDef spec pd))
-    where
-      npd = (rename_vars_ProcessDef1 (def_mem_st_Circus_aux spec) pd)
+    -- where
+      -- npd = (rename_vars_ProcessDef1 (def_mem_st_Circus_aux spec) pd)
 omega_ProcDecl spec (CProcess zn pd)
   = (CProcess zn (omega_ProcessDef spec pd))
-    where
-      npd = (rename_vars_ProcessDef1 (def_mem_st_Circus_aux spec) pd)
+    -- where
+      -- npd = (rename_vars_ProcessDef1 (def_mem_st_Circus_aux spec) pd)
 \end{code}
 
 \subsection{Mapping Circus Processes Definition}
@@ -198,7 +197,7 @@ omega_CProc spec (CRepSeqProc [(Choose x s)] a)
 omega_CProc spec (CSeq a b)
   = (CSeq (omega_CProc spec a) (omega_CProc spec b))
 omega_CProc spec (ProcStalessMain xls ca)
-  = (ProcStalessMain (concat (map (omega_PPar nstate) xls)) (mk_main_action_bind nstate (omega_CAction nstate ca)))
+  = (ProcStalessMain (concat (map omega_PPar xls)) (mk_main_action_bind nstate (omega_CAction ca)))
     where 
       nstate = (def_mem_st_Circus_aux spec)
 omega_CProc spec (CGenProc zn (x:xs))
@@ -211,15 +210,14 @@ omega_CProc spec (ProcMain zp (x:xs) ca)
   = (ProcStalessMain 
     [make_memory_proc] 
     (get_main_action 
-      (concat (map (omega_PPar nstate) (x:xs)))
-      (mk_main_action_bind nstate (omega_CAction nstate ca))))
+      (concat (map omega_PPar (x:xs)))
+      (mk_main_action_bind nstate (omega_CAction ca))))
     where 
       nstate = (def_mem_st_Circus_aux spec)
 omega_CProc spec x
   = x
 \end{code}
-Here I'm making the bindings for the main action. So far, I'm not implementing
-any invariants.
+Here I'm making the bindings for the main action. 
 \begin{code}
 mk_main_action_bind :: [(ZName, ZVar, ZExpr)] -> CAction -> CAction
 mk_main_action_bind lst ca
@@ -235,17 +233,17 @@ mk_inv ((a,b,ZVar c):xs)
 \end{code}
 \subsection{Mapping Parameterised Circus Actions}
 \begin{code}
-omega_PPar :: [(ZName, ZVar, ZExpr)] -> PPar -> [PPar]
-omega_PPar lst (ProcZPara zp) = [(ProcZPara zp)]
-omega_PPar lst (CParAction n pa) = [(CParAction n (omega_ParAction lst pa))]
-omega_PPar lst (CNameSet n ns) = [(CNameSet n ns)]
+omega_PPar :: PPar -> [PPar]
+omega_PPar (ProcZPara zp) = [(ProcZPara zp)]
+omega_PPar (CParAction n pa) = [(CParAction n (omega_ParAction pa))]
+omega_PPar (CNameSet n ns) = [(CNameSet n ns)]
 \end{code}
 \begin{code}
-omega_ParAction :: [(ZName, ZVar, ZExpr)] -> ParAction -> ParAction
-omega_ParAction lst (CircusAction ca)
-  = (CircusAction (omega_CAction lst ca))
-omega_ParAction lst (ParamActionDecl xl pa)
-  = (ParamActionDecl xl (omega_ParAction lst pa))
+omega_ParAction :: ParAction -> ParAction
+omega_ParAction (CircusAction ca)
+  = (CircusAction (omega_CAction ca))
+omega_ParAction (ParamActionDecl xl pa)
+  = (ParamActionDecl xl (omega_ParAction pa))
 \end{code}
 }
 \subsection{Stateless Circus - Actions}
@@ -257,10 +255,10 @@ omega_ParAction lst (ParamActionDecl xl pa)
 \end{circus}
 is written in Haskell as:
 \begin{code}
-omega_CAction :: [(ZName, ZVar, ZExpr)] -> CAction -> CAction
-omega_CAction lst CSPSkip = CSPSkip
-omega_CAction lst CSPStop = CSPStop
-omega_CAction lst CSPChaos = CSPChaos
+omega_CAction :: CAction -> CAction
+omega_CAction CSPSkip = CSPSkip
+omega_CAction CSPStop = CSPStop
+omega_CAction CSPChaos = CSPChaos
 \end{code}
 
 \begin{circus}
@@ -269,8 +267,8 @@ omega_CAction lst CSPChaos = CSPChaos
 
 is written in Haskell as:
 \begin{code}
-omega_CAction lst (CSPCommAction (ChanComm c []) a)
-  = (CSPCommAction (ChanComm c []) (omega_CAction lst a))
+omega_CAction (CSPCommAction (ChanComm c []) a)
+  = (CSPCommAction (ChanComm c []) (omega_CAction a))
 \end{code}
 
 \begin{circus}
@@ -286,9 +284,9 @@ FV (e) = (v_0,\ldots,v_n,l_0,\ldots,l_m)
 
 is written in Haskell as:
 \begin{code}
-omega_CAction lst (CSPCommAction (ChanComm c ((ChanDotExp e):xs)) a)
-  = make_get_com lst lxs (rename_vars_CAction (map fst lxs) (CSPCommAction (ChanComm c ((ChanDotExp e):xs)) (omega_prime_CAction lst a)))
-  where lxs = (get_chan_param ((ChanDotExp e):xs)) `intersect` (filter_state_comp lst)
+omega_CAction (CSPCommAction (ChanComm c ((ChanDotExp e):xs)) a)
+  = make_get_com lxs (rename_vars_CAction (CSPCommAction (ChanComm c ((ChanDotExp e):xs)) (omega_prime_CAction a)))
+  where lxs = concat (map get_ZVar_st (free_var_ZExpr e))
 \end{code}
 
 \begin{circus}
@@ -296,8 +294,8 @@ omega_CAction lst (CSPCommAction (ChanComm c ((ChanDotExp e):xs)) a)
 \\\t2 c.e(v_0,\ldots,v_n,l_0,\ldots,l_m) \then A
 \end{circus}
 \begin{code}
-omega_CAction lst (CSPCommAction (ChanComm c ((ChanOutExp e):xs)) a)
-  = omega_CAction lst (CSPCommAction (ChanComm c ((ChanDotExp e):xs)) a)
+omega_CAction (CSPCommAction (ChanComm c ((ChanOutExp e):xs)) a)
+  = omega_CAction (CSPCommAction (ChanComm c ((ChanDotExp e):xs)) a)
 \end{code}
 
 \begin{circus}
@@ -308,9 +306,9 @@ omega_CAction lst (CSPCommAction (ChanComm c ((ChanOutExp e):xs)) a)
 \end{circus}
 is written in Haskell as:
 \begin{code}
-omega_CAction lst (CSPGuard g a)
-  = make_get_com lst lxs (rename_vars_CAction (map fst lxs) (CSPGuard (rename_ZPred (map fst lxs) g) (omega_prime_CAction lst a)))
-  where lxs = nub $ free_var_ZPred(g) `intersect` (filter_state_comp lst)
+omega_CAction (CSPGuard g a)
+  = make_get_com lxs (rename_vars_CAction (CSPGuard (rename_ZPred g) (omega_prime_CAction a)))
+  where lxs = concat (map get_ZVar_st (free_var_ZPred g))
 \end{code}
 
 \begin{circus}
@@ -326,13 +324,13 @@ x \in wrtV(A)
 
 is written in Haskell as:
 \begin{code}
-omega_CAction lst (CSPCommAction (ChanComm c [ChanInpPred x p]) a)
+omega_CAction (CSPCommAction (ChanComm c [ChanInpPred x p]) a)
   = case not (elem x (getWrtV(a))) of
-    True -> make_get_com lst lsx (rename_vars_CAction (map fst lsx) (CSPCommAction
+    True -> make_get_com lsx (rename_vars_CAction (CSPCommAction
              (ChanComm c [ChanInpPred x p])
-                 (omega_prime_CAction lst a)))
+                 (omega_prime_CAction a)))
     _  -> (CSPCommAction (ChanComm c [ChanInpPred x p]) a)
-  where lsx = free_var_ZPred(p)
+  where lsx = concat (map get_ZVar_st (free_var_ZPred p))
 \end{code}
 
 
@@ -341,8 +339,8 @@ omega_CAction lst (CSPCommAction (ChanComm c [ChanInpPred x p]) a)
 \end{circus}
 is written in Haskell as:
 \begin{code}
-omega_CAction lst (CSPSeq ca cb)
-  = (CSPSeq (omega_CAction lst ca) (omega_CAction lst cb))
+omega_CAction (CSPSeq ca cb)
+  = (CSPSeq (omega_CAction ca) (omega_CAction cb))
 \end{code}
 
 \begin{circus}
@@ -350,8 +348,8 @@ omega_CAction lst (CSPSeq ca cb)
 \end{circus}
 is written in Haskell as:
 \begin{code}
-omega_CAction lst (CSPIntChoice ca cb)
-  = (CSPIntChoice (omega_CAction lst ca) (omega_CAction lst cb))
+omega_CAction (CSPIntChoice ca cb)
+  = (CSPIntChoice (omega_CAction ca) (omega_CAction cb))
 \end{code}
 
 % TODO: I need to somehow calculate the $FV(A_1)$ and $FV(A_2)$. What should I do?
@@ -363,10 +361,10 @@ omega_CAction lst (CSPIntChoice ca cb)
 \end{circus}
 is written in Haskell as:
 \begin{code}
-omega_CAction lst (CSPExtChoice ca cb)
-  = make_get_com lst lsx (rename_vars_CAction (map fst lsx) (CSPExtChoice (omega_prime_CAction lst ca) (omega_prime_CAction lst cb)))
+omega_CAction (CSPExtChoice ca cb)
+  = make_get_com lsx (rename_vars_CAction (CSPExtChoice (omega_prime_CAction ca) (omega_prime_CAction cb)))
    where
-    lsx = nub $ (free_var_CAction (CSPExtChoice ca cb)) `intersect` (filter_state_comp lst)
+    lsx = (map fst (nub (free_var_CAction (CSPExtChoice ca cb))))
 \end{code}
 
 \begin{circus}
@@ -400,8 +398,8 @@ omega_CAction lst (CSPExtChoice ca cb)
 \end{circus}
 
 \begin{code}
-omega_CAction lst (CSPNSParal ns1 cs ns2 a1 a2)
-  = make_get_com lst lsx (rename_vars_CAction (map fst lsx) (CSPHide
+omega_CAction (CSPNSParal ns1 cs ns2 a1 a2)
+  = make_get_com lsx (rename_vars_CAction (CSPHide
    (CSPNSParal NSExpEmpty (CSExpr "MEMi") NSExpEmpty
      (CSPNSParal NSExpEmpty cs NSExpEmpty
       (CSPHide
@@ -421,7 +419,7 @@ omega_CAction lst (CSPNSParal ns1 cs ns2 a1 a2)
       (CActionName "Merge"))
       (CChanSet ["mleft","mright"])))
    where
-    lsx = (free_var_CAction a1) `union` (free_var_CAction a2)
+    lsx = (map fst (nub (free_var_CAction a1))) `union` (map fst (nub (free_var_CAction a2)))
 \end{code}
 
 \begin{circus}
@@ -429,13 +427,13 @@ omega_CAction lst (CSPNSParal ns1 cs ns2 a1 a2)
 \end{circus}
 is written in Haskell as:
 \begin{code}
-omega_CAction lst (CSPRepSeq [Choose (x,[]) (ZSeqDisplay xs)] (CSPParAction act [ZVar (x1,[])]))
+omega_CAction (CSPRepSeq [Choose (x,[]) (ZSeqDisplay xs)] (CSPParAction act [ZVar (x1,[])]))
   = case x == x1 of
-    True -> omega_CAction lst (rep_CSPRepSeq lst act xs)
+    True -> omega_CAction (rep_CSPRepSeq act xs)
     _  -> (CSPRepSeq [Choose (x,[]) (ZSeqDisplay xs)]
-          (omega_CAction lst (CSPParAction act [ZVar (x1,[])])))
-omega_CAction lst (CSPRepSeq [Choose (x,[]) v] act)
-  = (CSPRepSeq [Choose (x,[]) v] (omega_CAction lst act))
+          (CSPParAction act [ZVar (x1,[])]))
+omega_CAction (CSPRepSeq [Choose (x,[]) v] act)
+  = (CSPRepSeq [Choose (x,[]) v] (omega_CAction act))
 \end{code}
 
 \begin{circus}
@@ -443,14 +441,13 @@ omega_CAction lst (CSPRepSeq [Choose (x,[]) v] act)
 \end{circus}
 is written in Haskell as:
 \begin{code}
-omega_CAction lst (CSPRepExtChoice [Choose (x,[]) (ZSeqDisplay xs)] (CSPParAction act [ZVar (x1,[])]))
+omega_CAction (CSPRepExtChoice [Choose (x,[]) (ZSeqDisplay xs)] (CSPParAction act [ZVar (x1,[])]))
   = case x == x1 of
-    True -> rep_CSPRepExtChoice lst act xs
+    True -> omega_CAction (rep_CSPRepExtChoice act xs)
     _  -> (CSPRepExtChoice [Choose (x,[]) (ZSeqDisplay xs)]
           (CSPParAction act [ZVar (x1,[])]))
-omega_CAction lst (CSPRepExtChoice [Choose (x,[]) v]
-          act)
-  = (CSPRepExtChoice [Choose (x,[]) v] (omega_CAction lst act))
+omega_CAction (CSPRepExtChoice [Choose (x,[]) v] act)
+  = (CSPRepExtChoice [Choose (x,[]) v] (omega_CAction act))
 \end{code}
 
 \begin{circus}
@@ -458,14 +455,14 @@ omega_CAction lst (CSPRepExtChoice [Choose (x,[]) v]
 \end{circus}
 is written in Haskell as:
 \begin{code}
-omega_CAction lst (CSPRepIntChoice [Choose (x,[]) (ZSeqDisplay xs)]
+omega_CAction (CSPRepIntChoice [Choose (x,[]) (ZSeqDisplay xs)]
           (CSPParAction act [ZVar (x1,[])]))
   = case x == x1 of
-    True -> rep_CSPRepIntChoice lst act xs
+    True -> omega_CAction(rep_CSPRepIntChoice act xs)
     _  -> (CSPRepIntChoice [Choose (x,[]) (ZSeqDisplay xs)]
           (CSPParAction act [ZVar (x1,[])]))
-omega_CAction lst (CSPRepIntChoice [Choose (x,[]) v] act)
-  = (CSPRepIntChoice [Choose (x,[]) v] (omega_CAction lst act))
+omega_CAction (CSPRepIntChoice [Choose (x,[]) v] act)
+  = (CSPRepIntChoice [Choose (x,[]) v] (omega_CAction act))
 \end{code}
 
 \begin{circus}
@@ -483,19 +480,19 @@ omega_CAction lst (CSPRepIntChoice [Choose (x,[]) v] act)
 \end{circus}
 is written in Haskell as:
 \begin{code}
-omega_CAction lst (CSPRepParalNS (CSExpr cs) [Choose (x,[]) (ZSetDisplay lsx)]
+omega_CAction (CSPRepParalNS (CSExpr cs) [Choose (x,[]) (ZSetDisplay lsx)]
           (NSExprParam ns [ZVar (x1,[])])
           (CSPParAction a [ZVar (x2,[])]))
   = case (x == x1) && (x == x2) of
-    True -> rep_CSPRepParalNS lst a cs ns x lsx
+    True -> omega_CAction (rep_CSPRepParalNS a cs ns x lsx)
     _  -> (CSPRepParalNS (CSExpr cs) [Choose (x,[]) (ZSetDisplay lsx)]
           (NSExprParam ns [ZVar (x1,[])])
-          (omega_CAction lst (CSPParAction a [ZVar (x2,[])])))
-omega_CAction lst (CSPRepParalNS (CSExpr cs) [Choose (x,[]) (ZSetDisplay lsx)]
+          (CSPParAction a [ZVar (x2,[])]))
+omega_CAction (CSPRepParalNS (CSExpr cs) [Choose (x,[]) (ZSetDisplay lsx)]
           (NSExprParam ns [ZVar (x1,[])]) act)
   = (CSPRepParalNS (CSExpr cs) [Choose (x,[]) (ZSetDisplay lsx)]
           (NSExprParam ns [ZVar (x1,[])])
-          (omega_CAction lst act))
+          (omega_CAction act))
 \end{code}
 % \begin{circus}
 % \Omega_A ( \circval Decl \circspot P) \circdef \circval Decl \circspot \Omega_A (P)
@@ -505,7 +502,6 @@ omega_CAction lst (CSPRepParalNS (CSExpr cs) [Choose (x,[]) (ZSetDisplay lsx)]
 % omega_CAction lst (CActionCommand (CValDecl xs a))
 %   = (CActionCommand (CValDecl xs (omega_CAction lst a)))
 % \end{code}
-(CActionCommand (CAssign [("time",[])] [ZCall (ZVar ("+",[])) (ZTuple [ZVar ("SysClock_time",[]),ZInt 1])]))
 \begin{circus}
 \Omega_A \left (\begin{array}{l}x_0,\ldots,x_n:=e_0\left (\begin{array}{l}v_0,...,v_n,\\l_0,...,l_m\end{array}\right ),\ldots,e_n\left (\begin{array}{l}v_0,...,v_n,\\l_0,...,l_m\end{array}\right )\end{array}\right ) \circdef
 \\\t1 get.v_0?vv_0 \then \ldots \then get.v_n?vv_n \then
@@ -516,8 +512,8 @@ omega_CAction lst (CSPRepParalNS (CSExpr cs) [Choose (x,[]) (ZSetDisplay lsx)]
 \end{circus}
 
 \begin{code}
-omega_CAction lst (CActionCommand (CAssign varls valls))
-= make_get_com lst varls (rename_vars_CAction (map fst (filter_state_comp lst)) (make_set_com lst varls valls CSPSkip))
+omega_CAction (CActionCommand (CAssign varls valls))
+  = make_get_com (map fst varls) (rename_vars_CAction (make_set_com varls valls CSPSkip))
 \end{code}
 \begin{circus}
 \Omega_A (\circif g (v_0,...,v_n,l_0,...,l_m) \circthen A \circfi ) \defs
@@ -526,11 +522,11 @@ omega_CAction lst (CActionCommand (CAssign varls valls))
    \\\t1\circif g (v_0,...,v_n,l_0,...,l_m) \circthen \Omega'_A (A) \circfi
 \end{circus}
 \begin{code}
-omega_CAction lst (CActionCommand (CIf (CircGAction g a)))
-  = make_get_com lst lsx (rename_vars_CAction (map fst lsx) (CActionCommand
-             (CIf (CircGAction g (omega_prime_CAction lst a)))))
+omega_CAction (CActionCommand (CIf (CircGAction g a)))
+  = make_get_com lsx (rename_vars_CAction  (CActionCommand
+             (CIf (CircGAction g (omega_prime_CAction a)))))
   where
-   lsx = free_var_ZPred g
+   lsx = (map fst (nub (free_var_ZPred g)))
 
 \end{code}
 \begin{circus}
@@ -550,11 +546,11 @@ omega_CAction lst (CActionCommand (CIf (CircGAction g a)))
 \end{circus}
 
 \begin{code}
-omega_CAction lst (CActionCommand (CIf (CircThenElse gl glx)))
-  = make_get_com lst lsx (rename_vars_CAction (map fst lsx) (CActionCommand (CIf (mk_guard_pair lst guard_pair))))
+omega_CAction (CActionCommand (CIf (CircThenElse gl glx)))
+  = make_get_com lsx (rename_vars_CAction (CActionCommand (CIf (mk_guard_pair guard_pair))))
   where
    guard_pair = get_guard_pair (CircThenElse gl glx)
-   lsx = nub $ concat $ map free_var_ZPred (map fst guard_pair)
+   lsx = map fst (remdups $ concat $ map free_var_ZPred (map fst guard_pair))
 \end{code}
 
 \begin{circus}
@@ -564,7 +560,7 @@ omega_CAction lst (CActionCommand (CIf (CircThenElse gl glx)))
 is written in Haskell as:
 
 \begin{code}
-omega_CAction lst (CSPHide a cs) = (CSPHide (omega_CAction lst a) cs)
+omega_CAction (CSPHide a cs) = (CSPHide (omega_CAction a) cs)
 \end{code}
 
 \begin{circus}
@@ -574,7 +570,7 @@ omega_CAction lst (CSPHide a cs) = (CSPHide (omega_CAction lst a) cs)
 is written in Haskell as:
 
 \begin{code}
-omega_CAction lst (CSPRecursion x c) = (CSPRecursion x (omega_CAction lst c))
+omega_CAction (CSPRecursion x c) = (CSPRecursion x (omega_CAction c))
 \end{code}
 
 \begin{circus}
@@ -594,20 +590,20 @@ omega_CAction lst (CSPRecursion x c) = (CSPRecursion x (omega_CAction lst c))
 is written in Haskell as:
 
 \begin{code}
-omega_CAction lst (CSPRepInterlNS [Choose (x,[]) (ZSetDisplay lsx)]
+omega_CAction (CSPRepInterlNS [Choose (x,[]) (ZSetDisplay lsx)]
           (NSExprParam ns [ZVar (x1,[])])
           (CSPParAction a [ZVar (x2,[])]))
   = case (x == x1) && (x == x2) of
-    True -> rep_CSPRepInterlNS lst a ns x lsx
+    True -> omega_CAction (rep_CSPRepInterlNS a ns x lsx)
     _  ->  (CSPRepInterlNS [Choose (x,[]) (ZSetDisplay lsx)]
           (NSExprParam ns [ZVar (x1,[])])
-          (omega_CAction lst (CSPParAction a [ZVar (x2,[])])))
-omega_CAction lst (CSPRepInterlNS [Choose (x,[]) (ZSetDisplay lsx)]
+          (CSPParAction a [ZVar (x2,[])]))
+omega_CAction (CSPRepInterlNS [Choose (x,[]) (ZSetDisplay lsx)]
           (NSExprParam ns [ZVar (x1,[])])
           act)
   = (CSPRepInterlNS [Choose (x,[]) (ZSetDisplay lsx)]
           (NSExprParam ns [ZVar (x1,[])])
-          (omega_CAction lst act))
+          (omega_CAction act))
 \end{code}
 
 \begin{circus}
@@ -615,8 +611,8 @@ omega_CAction lst (CSPRepInterlNS [Choose (x,[]) (ZSetDisplay lsx)]
 \end{circus}
 
 \begin{code}
-omega_CAction lst (CActionCommand (CommandBrace g))
-  = omega_CAction lst (CActionCommand (CPrefix g (ZTrue {reason = []})))
+omega_CAction (CActionCommand (CommandBrace g))
+  = omega_CAction (CActionCommand (CPrefix g (ZTrue {reason = []})))
 \end{code}
 
 \begin{circus}
@@ -624,8 +620,8 @@ omega_CAction lst (CActionCommand (CommandBrace g))
 \end{circus}
 
 \begin{code}
-omega_CAction lst (CActionCommand (CommandBracket g))
-  = omega_CAction lst (CActionCommand (CPrefix1 g))
+omega_CAction (CActionCommand (CommandBracket g))
+  = omega_CAction (CActionCommand (CPrefix1 g))
 \end{code}
 
 \begin{circus}
@@ -634,9 +630,9 @@ omega_CAction lst (CActionCommand (CommandBracket g))
 \end{circus}
 
 \begin{code}
-omega_CAction lst (CSPRenAction a (CRenameAssign left right))
+omega_CAction (CSPRenAction a (CRenameAssign left right))
   = (CSPRenAction a (CRename right left))
-omega_CAction lst x = x
+omega_CAction x = x
 \end{code}
 
 
@@ -645,10 +641,10 @@ NOTE: Besides the transformation rules for $[g]$ and ${g}$, the remaining transf
 
 
 \begin{code}
-omega_prime_CAction :: [(ZName, ZVar, ZExpr)] -> CAction -> CAction
-omega_prime_CAction lst CSPSkip = CSPSkip
-omega_prime_CAction lst CSPStop = CSPStop
-omega_prime_CAction lst CSPChaos = CSPChaos
+omega_prime_CAction :: CAction -> CAction
+omega_prime_CAction CSPSkip = CSPSkip
+omega_prime_CAction CSPStop = CSPStop
+omega_prime_CAction CSPChaos = CSPChaos
 \end{code}
 
 \begin{circus}
@@ -657,8 +653,8 @@ omega_prime_CAction lst CSPChaos = CSPChaos
 
 is written in Haskell as:
 \begin{code}
-omega_prime_CAction lst (CSPCommAction (ChanComm c []) a)
-  = (CSPCommAction (ChanComm c []) (omega_prime_CAction lst a))
+omega_prime_CAction (CSPCommAction (ChanComm c []) a)
+  = (CSPCommAction (ChanComm c []) (omega_prime_CAction a))
 \end{code}
 
 \begin{circus}
@@ -667,8 +663,8 @@ omega_prime_CAction lst (CSPCommAction (ChanComm c []) a)
 
 is written in Haskell as:
 \begin{code}
-omega_prime_CAction lst (CSPCommAction (ChanComm c x) a)
-  = (CSPCommAction (ChanComm c x) (omega_prime_CAction lst a))
+omega_prime_CAction (CSPCommAction (ChanComm c x) a)
+  = (CSPCommAction (ChanComm c x) (omega_prime_CAction a))
 \end{code}
 
 \begin{circus}
@@ -677,8 +673,8 @@ omega_prime_CAction lst (CSPCommAction (ChanComm c x) a)
 \end{circus}
 is written in Haskell as:
 \begin{code}
-omega_prime_CAction lst (CSPGuard g a)
-  = (CSPGuard g (omega_prime_CAction lst a))
+omega_prime_CAction (CSPGuard g a)
+  = (CSPGuard g (omega_prime_CAction a))
 \end{code}
 
 
@@ -687,8 +683,8 @@ omega_prime_CAction lst (CSPGuard g a)
 \end{circus}
 is written in Haskell as:
 \begin{code}
-omega_prime_CAction lst (CSPSeq ca cb)
-  = (CSPSeq (omega_prime_CAction lst ca) (omega_prime_CAction lst cb))
+omega_prime_CAction (CSPSeq ca cb)
+  = (CSPSeq (omega_prime_CAction ca) (omega_prime_CAction cb))
 \end{code}
 
 \begin{circus}
@@ -696,8 +692,8 @@ omega_prime_CAction lst (CSPSeq ca cb)
 \end{circus}
 is written in Haskell as:
 \begin{code}
-omega_prime_CAction lst (CSPIntChoice ca cb)
-  = (CSPIntChoice (omega_prime_CAction lst ca) (omega_prime_CAction lst cb))
+omega_prime_CAction (CSPIntChoice ca cb)
+  = (CSPIntChoice (omega_prime_CAction ca) (omega_prime_CAction cb))
 \end{code}
 
 % TODO: I need to somehow calculate the $FV(A_1)$ and $FV(A_2)$. What should I do?
@@ -709,10 +705,10 @@ omega_prime_CAction lst (CSPIntChoice ca cb)
 \end{circus}
 is written in Haskell as:
 \begin{code}
-omega_prime_CAction lst (CSPExtChoice ca cb)
-  = make_get_com lst lsx (CSPExtChoice (omega_prime_CAction lst ca) (omega_prime_CAction lst cb))
+omega_prime_CAction (CSPExtChoice ca cb)
+  = make_get_com lsx (CSPExtChoice (omega_prime_CAction ca) (omega_prime_CAction cb))
    where
-    lsx = nub $ (free_var_CAction (CSPExtChoice ca cb)) `intersect` (filter_state_comp lst)
+    lsx = concat (map get_ZVar_st (remdups (free_var_CAction (CSPExtChoice ca cb))) )
 \end{code}
 
 \begin{circus}
@@ -746,8 +742,8 @@ omega_prime_CAction lst (CSPExtChoice ca cb)
 \end{circus}
 
 \begin{code}
-omega_prime_CAction lst (CSPNSParal ns1 cs ns2 a1 a2)
-  = make_get_com lst lsx (CSPHide
+omega_prime_CAction (CSPNSParal ns1 cs ns2 a1 a2)
+  = make_get_com lsx (CSPHide
    (CSPNSParal NSExpEmpty (CSExpr "MEMi") NSExpEmpty
      (CSPNSParal NSExpEmpty cs NSExpEmpty
       (CSPHide
@@ -767,7 +763,7 @@ omega_prime_CAction lst (CSPNSParal ns1 cs ns2 a1 a2)
       (CActionName "Merge"))
       (CChanSet ["mleft","mright"]))
    where
-    lsx = (free_var_CAction a1) `union` (free_var_CAction a2)
+    lsx = concat (map get_ZVar_st ((free_var_CAction a1) `union` (free_var_CAction a2)))
 \end{code}
 
 \begin{circus}
@@ -775,13 +771,13 @@ omega_prime_CAction lst (CSPNSParal ns1 cs ns2 a1 a2)
 \end{circus}
 is written in Haskell as:
 \begin{code}
-omega_prime_CAction lst (CSPRepSeq [Choose (x,[]) (ZSeqDisplay xs)] (CSPParAction act [ZVar (x1,[])]))
+omega_prime_CAction (CSPRepSeq [Choose (x,[]) (ZSeqDisplay xs)] (CSPParAction act [ZVar (x1,[])]))
   = case x == x1 of
-    True -> omega_prime_CAction lst (rep_CSPRepSeq lst act xs)
+    True -> omega_prime_CAction (rep_CSPRepSeq act xs)
     _  -> (CSPRepSeq [Choose (x,[]) (ZSeqDisplay xs)]
-          (omega_prime_CAction lst (CSPParAction act [ZVar (x1,[])])))
-omega_prime_CAction lst (CSPRepSeq [Choose (x,[]) v] act)
-  = (CSPRepSeq [Choose (x,[]) v] (omega_prime_CAction lst act))
+          (CSPParAction act [ZVar (x1,[])]))
+omega_prime_CAction (CSPRepSeq [Choose (x,[]) v] act)
+  = (CSPRepSeq [Choose (x,[]) v] (omega_prime_CAction act))
 \end{code}
 
 \begin{circus}
@@ -789,14 +785,13 @@ omega_prime_CAction lst (CSPRepSeq [Choose (x,[]) v] act)
 \end{circus}
 is written in Haskell as:
 \begin{code}
-omega_prime_CAction lst (CSPRepExtChoice [Choose (x,[]) (ZSeqDisplay xs)] (CSPParAction act [ZVar (x1,[])]))
+omega_prime_CAction (CSPRepExtChoice [Choose (x,[]) (ZSeqDisplay xs)] (CSPParAction act [ZVar (x1,[])]))
   = case x == x1 of
-    True -> rep_CSPRepExtChoice lst act xs
+    True -> omega_CAction (rep_CSPRepExtChoice act xs)
     _  -> (CSPRepExtChoice [Choose (x,[]) (ZSeqDisplay xs)]
           (CSPParAction act [ZVar (x1,[])]))
-omega_prime_CAction lst (CSPRepExtChoice [Choose (x,[]) v]
-          act)
-  = (CSPRepExtChoice [Choose (x,[]) v] (omega_prime_CAction lst act))
+omega_prime_CAction (CSPRepExtChoice [Choose (x,[]) v] act)
+  = (CSPRepExtChoice [Choose (x,[]) v] (omega_prime_CAction act))
 \end{code}
 
 \begin{circus}
@@ -804,14 +799,14 @@ omega_prime_CAction lst (CSPRepExtChoice [Choose (x,[]) v]
 \end{circus}
 is written in Haskell as:
 \begin{code}
-omega_prime_CAction lst (CSPRepIntChoice [Choose (x,[]) (ZSeqDisplay xs)]
+omega_prime_CAction (CSPRepIntChoice [Choose (x,[]) (ZSeqDisplay xs)]
           (CSPParAction act [ZVar (x1,[])]))
   = case x == x1 of
-    True -> rep_CSPRepIntChoice lst act xs
+    True -> omega_CAction (rep_CSPRepIntChoice act xs)
     _  -> (CSPRepIntChoice [Choose (x,[]) (ZSeqDisplay xs)]
           (CSPParAction act [ZVar (x1,[])]))
-omega_prime_CAction lst (CSPRepIntChoice [Choose (x,[]) v] act)
-  = (CSPRepIntChoice [Choose (x,[]) v] (omega_prime_CAction lst act))
+omega_prime_CAction (CSPRepIntChoice [Choose (x,[]) v] act)
+  = (CSPRepIntChoice [Choose (x,[]) v] (omega_prime_CAction act))
 \end{code}
 
 \begin{circus}
@@ -829,19 +824,16 @@ omega_prime_CAction lst (CSPRepIntChoice [Choose (x,[]) v] act)
 \end{circus}
 is written in Haskell as:
 \begin{code}
-omega_prime_CAction lst (CSPRepParalNS (CSExpr cs) [Choose (x,[]) (ZSetDisplay lsx)]
-          (NSExprParam ns [ZVar (x1,[])])
-          (CSPParAction a [ZVar (x2,[])]))
-  = case (x == x1) && (x == x2) of
-    True -> rep_CSPRepParalNS lst a cs ns x lsx
-    _  -> (CSPRepParalNS (CSExpr cs) [Choose (x,[]) (ZSetDisplay lsx)]
-          (NSExprParam ns [ZVar (x1,[])])
-          (omega_prime_CAction lst (CSPParAction a [ZVar (x2,[])])))
-omega_prime_CAction lst (CSPRepParalNS (CSExpr cs) [Choose (x,[]) (ZSetDisplay lsx)]
-          (NSExprParam ns [ZVar (x1,[])]) act)
+omega_prime_CAction (CSPRepParalNS (CSExpr cs) [Choose (x,[]) (ZSetDisplay lsx)] (NSExprParam ns [ZVar (x1,[])]) (CSPParAction a [ZVar (x2,[])]))
+  = case (x == x1) && (x == x2) of 
+      True -> omega_CAction (rep_CSPRepParalNS a cs ns x lsx) 
+      _  -> (CSPRepParalNS (CSExpr cs) [Choose (x,[]) (ZSetDisplay lsx)] 
+              (NSExprParam ns [ZVar (x1,[])]) (omega_prime_CAction (CSPParAction a [ZVar (x2,[])])))
+
+omega_prime_CAction (CSPRepParalNS (CSExpr cs) [Choose (x,[]) (ZSetDisplay lsx)] (NSExprParam ns [ZVar (x1,[])]) act)
   = (CSPRepParalNS (CSExpr cs) [Choose (x,[]) (ZSetDisplay lsx)]
           (NSExprParam ns [ZVar (x1,[])])
-          (omega_prime_CAction lst act))
+          (omega_prime_CAction act))
 \end{code}
 \begin{circus}
 \Omega'_A \left (\begin{array}{l}x_0,\ldots,x_n:=e_0\left (\begin{array}{l}v_0,...,v_n,\\l_0,...,l_m\end{array}\right ),\ldots,e_n\left (\begin{array}{l}v_0,...,v_n,\\l_0,...,l_m\end{array}\right )\end{array}\right ) \circdef
@@ -851,8 +843,8 @@ omega_prime_CAction lst (CSPRepParalNS (CSExpr cs) [Choose (x,[]) (ZSetDisplay l
 \end{circus}
 
 \begin{code}
-omega_prime_CAction lst (CActionCommand (CAssign varls valls))
-  = (make_set_com lst varls valls CSPSkip)
+omega_prime_CAction (CActionCommand (CAssign varls valls))
+  = (make_set_com varls valls CSPSkip)
 \end{code}
 
 \begin{circus}
@@ -861,8 +853,8 @@ omega_prime_CAction lst (CActionCommand (CAssign varls valls))
    \\\t1\circif g (v_0,...,v_n,l_0,...,l_m) \circthen \Omega'_A (A) \circfi
 \end{circus}
 \begin{code}
-omega_prime_CAction lst (CActionCommand (CIf (CircGAction g a)))
-  = (CActionCommand (CIf (CircGAction g (omega_prime_CAction lst a))))
+omega_prime_CAction (CActionCommand (CIf (CircGAction g a)))
+  = (CActionCommand (CIf (CircGAction g (omega_prime_CAction a))))
 
 \end{code}
 \begin{circus}
@@ -880,8 +872,8 @@ omega_prime_CAction lst (CActionCommand (CIf (CircGAction g a)))
 \end{circus}
 
 \begin{code}
-omega_prime_CAction lst (CActionCommand (CIf (CircThenElse gl glx)))
-  = (CActionCommand (CIf (mk_guard_pair lst guard_pair)))
+omega_prime_CAction (CActionCommand (CIf (CircThenElse gl glx)))
+  = (CActionCommand (CIf (mk_guard_pair guard_pair)))
   where
    guard_pair = get_guard_pair (CircThenElse gl glx)
 \end{code}
@@ -893,7 +885,7 @@ omega_prime_CAction lst (CActionCommand (CIf (CircThenElse gl glx)))
 is written in Haskell as:
 
 \begin{code}
-omega_prime_CAction lst (CSPHide a cs) = (CSPHide (omega_prime_CAction lst a) cs)
+omega_prime_CAction (CSPHide a cs) = (CSPHide (omega_prime_CAction a) cs)
 \end{code}
 
 \begin{circus}
@@ -903,7 +895,7 @@ omega_prime_CAction lst (CSPHide a cs) = (CSPHide (omega_prime_CAction lst a) cs
 is written in Haskell as:
 
 \begin{code}
-omega_prime_CAction lst (CSPRecursion x c) = (CSPRecursion x (omega_prime_CAction lst c))
+omega_prime_CAction (CSPRecursion x c) = (CSPRecursion x (omega_prime_CAction c))
 \end{code}
 
 \begin{circus}
@@ -923,20 +915,20 @@ omega_prime_CAction lst (CSPRecursion x c) = (CSPRecursion x (omega_prime_CActio
 is written in Haskell as:
 
 \begin{code}
-omega_prime_CAction lst (CSPRepInterlNS [Choose (x,[]) (ZSetDisplay lsx)]
+omega_prime_CAction (CSPRepInterlNS [Choose (x,[]) (ZSetDisplay lsx)]
           (NSExprParam ns [ZVar (x1,[])])
           (CSPParAction a [ZVar (x2,[])]))
   = case (x == x1) && (x == x2) of
-    True -> rep_CSPRepInterlNS lst a ns x lsx
+    True -> omega_CAction (rep_CSPRepInterlNS a ns x lsx)
     _  ->  (CSPRepInterlNS [Choose (x,[]) (ZSetDisplay lsx)]
           (NSExprParam ns [ZVar (x1,[])])
-          (omega_prime_CAction lst (CSPParAction a [ZVar (x2,[])])))
-omega_prime_CAction lst (CSPRepInterlNS [Choose (x,[]) (ZSetDisplay lsx)]
+          (CSPParAction a [ZVar (x2,[])]))
+omega_prime_CAction (CSPRepInterlNS [Choose (x,[]) (ZSetDisplay lsx)]
           (NSExprParam ns [ZVar (x1,[])])
           act)
   = (CSPRepInterlNS [Choose (x,[]) (ZSetDisplay lsx)]
           (NSExprParam ns [ZVar (x1,[])])
-          (omega_prime_CAction lst act))
+          (omega_prime_CAction act))
 \end{code}
 
 \begin{circus}
@@ -944,8 +936,8 @@ omega_prime_CAction lst (CSPRepInterlNS [Choose (x,[]) (ZSetDisplay lsx)]
 \end{circus}
 
 \begin{code}
-omega_prime_CAction lst (CActionCommand (CommandBrace g))
-  = omega_prime_CAction lst (CActionCommand (CPrefix g (ZTrue {reason = []})))
+omega_prime_CAction (CActionCommand (CommandBrace g))
+  = omega_prime_CAction (CActionCommand (CPrefix g (ZTrue {reason = []})))
 \end{code}
 
 \begin{circus}
@@ -953,8 +945,8 @@ omega_prime_CAction lst (CActionCommand (CommandBrace g))
 \end{circus}
 
 \begin{code}
-omega_prime_CAction lst (CActionCommand (CommandBracket g))
-  = omega_prime_CAction lst (CActionCommand (CPrefix1 g))
+omega_prime_CAction (CActionCommand (CommandBracket g))
+  = omega_prime_CAction (CActionCommand (CPrefix1 g))
 \end{code}
 
 \begin{circus}
@@ -963,76 +955,79 @@ omega_prime_CAction lst (CActionCommand (CommandBracket g))
 \end{circus}
 
 \begin{code}
-omega_prime_CAction lst (CSPRenAction a (CRenameAssign left right))
+omega_prime_CAction (CSPRenAction a (CRenameAssign left right))
   = (CSPRenAction a (CRename right left))
 \end{code}
 
 \begin{code}
-omega_prime_CAction lst (CActionName n)
+omega_prime_CAction (CActionName n)
   = (CActionName n)
 \end{code}
 
 \begin{code}
-omega_prime_CAction lst x 
+omega_prime_CAction x 
   = error ("Not defined for Omega'"++ show x)
 \end{code}
 \subsection{Auxiliary functions for the definition of $\Omega_{A}$}
+The use of Isabelle/HOL made me rethink of what was being produced
+with the functions below. First, a $CSPParAction$, $A(x)$, does not need to call $omega_CAction$ again, as it does not change anything, so I removed it when a list of parameters $x$ is a singleton. Then, I realised that I don't need to call $omega_CAction$ at all in any of the $rep\_$ functions as that function is called for the result of any $rep\_$ function. Finally, I don't need to carry the triple with the state variable names/types. 
+
 Function used to propagate $CSPRepSeq$ actions
 
 \begin{code}
-rep_CSPRepSeq :: [(ZName, ZVar, ZExpr)] -> ZName -> [ZExpr] -> CAction
-rep_CSPRepSeq lst a [x]
-  = omega_CAction lst (CSPParAction a [x])
-rep_CSPRepSeq lst a (x:xs)
-  = CSPSeq (omega_CAction lst (CSPParAction a [x])) (rep_CSPRepSeq lst a xs)
+rep_CSPRepSeq :: ZName -> [ZExpr] -> CAction
+rep_CSPRepSeq a [x]
+  = (CSPParAction a [x])
+rep_CSPRepSeq a (x:xs)
+  = CSPSeq (CSPParAction a [x]) (rep_CSPRepSeq a xs)
 \end{code}
 
 Function used to propagate $CSPRepIntChoice$ actions
 
 \begin{code}
-rep_CSPRepIntChoice :: [(ZName, ZVar, ZExpr)] -> ZName -> [ZExpr] -> CAction
-rep_CSPRepIntChoice lst a [x]
-  = omega_CAction lst (CSPParAction a [x])
-rep_CSPRepIntChoice lst a (x:xs)
-  = CSPIntChoice (omega_CAction lst (CSPParAction a [x])) (rep_CSPRepIntChoice lst a xs)
+rep_CSPRepIntChoice :: ZName -> [ZExpr] -> CAction
+rep_CSPRepIntChoice a [x]
+  = (CSPParAction a [x])
+rep_CSPRepIntChoice a (x:xs)
+  = CSPIntChoice (CSPParAction a [x]) (rep_CSPRepIntChoice a xs)
 \end{code}
 
 Function used to propagate $CSPRepExtChoice$ actions
 
 \begin{code}
-rep_CSPRepExtChoice :: [(ZName, ZVar, ZExpr)] -> ZName -> [ZExpr] -> CAction
-rep_CSPRepExtChoice lst a [x]
-  =  omega_CAction lst (CSPParAction a [x])
-rep_CSPRepExtChoice lst a (x:xs)
-  = CSPExtChoice ( omega_CAction lst (CSPParAction a [x])) (rep_CSPRepExtChoice lst a xs)
+rep_CSPRepExtChoice :: ZName -> [ZExpr] -> CAction
+rep_CSPRepExtChoice a [x]
+  = (CSPParAction a [x])
+rep_CSPRepExtChoice a (x:xs)
+  = CSPExtChoice (CSPParAction a [x]) (rep_CSPRepExtChoice a xs)
 \end{code}
 
 Function used to propagate $CSPRepInterNS$ actions
 
 \begin{code}
-rep_CSPRepParalNS :: [(ZName, ZVar, ZExpr)] -> ZName -> ZName -> ZName -> String -> [ZExpr] -> CAction
-rep_CSPRepParalNS lst a _ _ _ [x]
-  =  omega_CAction lst (CSPParAction a [x])
-rep_CSPRepParalNS lst a cs ns y (x:xs)
+rep_CSPRepParalNS :: ZName -> ZName -> ZName -> String -> [ZExpr] -> CAction
+rep_CSPRepParalNS a _ _ _ [x]
+  = (CSPParAction a [x])
+rep_CSPRepParalNS a cs ns y (x:xs)
   = (CSPNSParal (NSExprParam ns [x]) (CSExpr cs)
     (NSBigUnion (ZSetComp
            [Choose (y,[]) (ZSetDisplay xs)]
            (Just (ZCall (ZVar (ns,[])) (ZVar (y,[])))) ) )
-     ( omega_CAction lst (CSPParAction a [x])) (rep_CSPRepParalNS lst a cs ns y xs) )
+     (CSPParAction a [x]) (rep_CSPRepParalNS a cs ns y xs) )
 \end{code}
 
 Function used to propagate $CSPRepInterNS$ actions
 
 \begin{code}
-rep_CSPRepInterlNS :: [(ZName, ZVar, ZExpr)] -> ZName -> ZName -> String -> [ZExpr] -> CAction
-rep_CSPRepInterlNS lst a _ _ [x]
-  =  omega_CAction lst (CSPParAction a [x])
-rep_CSPRepInterlNS lst a ns y (x:xs)
+rep_CSPRepInterlNS :: ZName -> ZName -> String -> [ZExpr] -> CAction
+rep_CSPRepInterlNS a _ _ [x]
+  = (CSPParAction a [x])
+rep_CSPRepInterlNS a ns y (x:xs)
   = (CSPNSInter (NSExprParam ns [x])
     (NSBigUnion (ZSetComp
            [Choose (y,[]) (ZSetDisplay xs)]
            (Just (ZCall (ZVar (ns,[])) (ZVar (y,[])))) ) )
-     ( omega_CAction lst (CSPParAction a [x])) (rep_CSPRepInterlNS lst a ns y xs) )
+     (CSPParAction a [x]) (rep_CSPRepInterlNS a ns y xs) )
 \end{code}
 
 Auxiliary function to propagate $get$ communication through the variables and local variables of an action.
@@ -1042,24 +1037,24 @@ make\_get\_com\ (v_0,\ldots,v_n,l_0,\ldots,l_m)~A \defs
 \\\t2 get.l_0?vl_0 \then \ldots \then get.l_m?vl_m \then A
 \end{circus}
 \begin{code}
-make_get_com :: [(ZName, ZVar, ZExpr)] -> [ZVar] -> CAction -> CAction
-make_get_com lst [(x,[])] c
+make_get_com :: [ZName] -> CAction -> CAction
+make_get_com [x] c
   = (CSPCommAction (ChanComm "mget"
-    [ChanDotExp (ZVar ((get_proc_name x lst)++"_"++x,[])),ChanInp ("v"++(get_proc_name x lst)++"_"++x)]) c)
-make_get_com lst ((x,[]):xs) c
+    [ChanDotExp (ZVar (x,[])),ChanInp ("v_"++x)]) c)
+make_get_com (x:xs) c
   = (CSPCommAction (ChanComm "mget"
-    [ChanDotExp (ZVar ((get_proc_name x lst)++"_"++x,[])),ChanInp ("v"++(get_proc_name x lst)++"_"++x)]) (make_get_com lst xs c))
-make_get_com lst x c = c    
+    [ChanDotExp (ZVar (x,[])),ChanInp ("v_"++x)]) (make_get_com xs c))
+make_get_com x c = c    
 \end{code}
 
 \begin{code}
-make_set_com :: [(ZName, ZVar, ZExpr)] -> [ZVar] -> [ZExpr] -> CAction -> CAction
-make_set_com lst [(x,[])] [y] c
+make_set_com :: [ZVar] -> [ZExpr] -> CAction -> CAction
+make_set_com [(x,_)] [y] c
   = (CSPCommAction (ChanComm "mset"
-    [ChanDotExp (ZVar ((get_proc_name x lst)++"_"++x,[])),ChanOutExp y]) (omega_CAction lst c))
-make_set_com lst (((x,[])):xs) (y:ys) c
+    [ChanDotExp (ZVar (x,[])),ChanOutExp y]) (omega_CAction c))
+make_set_com ((x,_):xs) (y:ys) c
   = (CSPCommAction (ChanComm "mset"
-     [ChanDotExp (ZVar ((get_proc_name x lst)++"_"++x,[])),ChanOutExp y]) (make_set_com lst xs ys c))
+     [ChanDotExp (ZVar (x,[])),ChanOutExp y]) (make_set_com xs ys c))
 \end{code}
 
 Given $\{v_0,\ldots,v_n\}$, the function $make\_maps\_to$ returns $\{v_0 \mapsto vv_o, \ldots, v_n \mapsto vv_n\}$.
@@ -1067,10 +1062,10 @@ Given $\{v_0,\ldots,v_n\}$, the function $make\_maps\_to$ returns $\{v_0 \mapsto
 make_maps_to :: [ZVar] -> [ZExpr]
 make_maps_to [(x,[])]
   = [ZCall (ZVar ("\\mapsto",[]))
-    (ZTuple [ZVar (x,[]),ZVar ("v"++x,[])])]
+    (ZTuple [ZVar (x,[]),ZVar ("val"++x,[])])]
 make_maps_to ((x,[]):xs)
   = [ZCall (ZVar ("\\mapsto",[]))
-    (ZTuple [ZVar (x,[]),ZVar ("v"++x,[])])]++(make_maps_to xs)
+    (ZTuple [ZVar (x,[]),ZVar ("val"++x,[])])]++(make_maps_to xs)
 \end{code}
 
 The function $get\_guard\_pair$ transform $CircGAction$ constructs into a list of tuples $(ZPred, CAction)$
@@ -1084,11 +1079,11 @@ get_guard_pair (CircThenElse (CircGAction g1 a1) glx)
 
 The function $mk\_guard\_pair$ transforms a list of tuples $(ZPred, CAction)$ and produces $CircThenElse$ pieces according to the size of the list.
 \begin{code}
-mk_guard_pair :: [(ZName, ZVar, ZExpr)] -> [(ZPred, CAction)] -> CGActions
-mk_guard_pair lst [(g,a)]
-  = (CircGAction g (omega_prime_CAction lst a))
-mk_guard_pair lst ((g,a):ls)
-  = (CircThenElse (CircGAction g (omega_prime_CAction lst a)) (mk_guard_pair lst ls))
+mk_guard_pair :: [(ZPred, CAction)] -> CGActions
+mk_guard_pair [(g,a)]
+  = (CircGAction g (omega_prime_CAction a))
+mk_guard_pair ((g,a):ls)
+  = (CircThenElse (CircGAction g (omega_prime_CAction a)) (mk_guard_pair ls))
 \end{code}
 % \subsection{Adding permanent bits of the new \Circus specification ($MemoryMerge$, $MRG$, etc)}
 
