test_haskabelle/MappingFunStatelessCircus.hs
@@ -12,223 +12,160 @@ module MappingFunStatelessCircus
 where
 import AST
 import OmegaDefs
--- import DefSets
--- import Data.List
--- import FormatterToCSP
 
-omega_CAction :: [(ZName, ZVar, ZExpr)] -> CAction -> CAction
-omega_CAction lst CSPSkip = CSPSkip
-omega_CAction lst CSPStop = CSPStop
-omega_CAction lst CSPChaos = CSPChaos
-omega_CAction lst (CSPCommAction (ChanComm c ((ChanOutExp e):xs)) a) = omega_CAction lst (CSPCommAction (ChanComm c ((ChanDotExp e):xs)) a)
-omega_CAction lst (CSPSeq ca cb) = (CSPSeq (omega_CAction lst ca) (omega_CAction lst cb))
-omega_CAction lst (CSPIntChoice ca cb) = (CSPIntChoice (omega_CAction lst ca) (omega_CAction lst cb))
-omega_CAction lst (CSPCommAction (ChanComm c []) a) = (CSPCommAction (ChanComm c []) (omega_CAction lst a))
-omega_CAction lst (CSPHide a cs) = (CSPHide (omega_CAction lst a) cs)
-omega_CAction lst (CSPRecursion x c) = (CSPRecursion x (omega_CAction lst c))
-omega_CAction lst (CActionCommand (CommandBrace g)) = omega_CAction lst (CActionCommand (CPrefix g (ZTrue {reason = []})))
-omega_CAction lst (CActionCommand (CommandBracket g)) = omega_CAction lst (CActionCommand (CPrefix1 g))
-omega_CAction lst (CSPRenAction a (CRenameAssign left right)) = (CSPRenAction a (CRename right left))
-omega_CAction lst (CSPRepSeq [Choose (x,[]) (ZSeqDisplay xs)] (CSPParAction act [ZVar (x1,[])]))
-  = case x == x1 of
-    True -> omega_CAction lst (rep_CSPRepSeq lst omega_CAction act xs)
-    _  -> (CSPRepSeq [Choose (x,[]) (ZSeqDisplay xs)]
-          (omega_CAction lst (CSPParAction act [ZVar (x1,[])])))
-omega_CAction lst (CSPRepSeq [Choose (x,[]) v] act)
-  = (CSPRepSeq [Choose (x,[]) v] (omega_CAction lst act))
 
-omega_CAction lst (CSPRepExtChoice [Choose (x,[]) (ZSeqDisplay xs)] (CSPParAction act [ZVar (x1,[])]))
-  = case x == x1 of
-    True -> rep_CSPRepExtChoice lst omega_CAction act xs
-    _  -> (CSPRepExtChoice [Choose (x,[]) (ZSeqDisplay xs)]
-          (CSPParAction act [ZVar (x1,[])]))
-omega_CAction lst (CSPRepExtChoice [Choose (x,[]) v] act)
-  = (CSPRepExtChoice [Choose (x,[]) v] (omega_CAction lst act))
+omega_CAction :: CAction -> CAction
+omega_CAction CSPSkip = CSPSkip
+omega_CAction CSPStop = CSPStop
+omega_CAction CSPChaos = CSPChaos
 
-omega_CAction lst (CSPRepIntChoice [Choose (x,[]) (ZSeqDisplay xs)]
-          (CSPParAction act [ZVar (x1,[])]))
-  = case x == x1 of
-    True -> rep_CSPRepIntChoice lst omega_CAction act xs
-    _  -> (CSPRepIntChoice [Choose (x,[]) (ZSeqDisplay xs)]
-          (CSPParAction act [ZVar (x1,[])]))
-omega_CAction lst (CSPRepIntChoice [Choose (x,[]) v] act)
-  = (CSPRepIntChoice [Choose (x,[]) v] (omega_CAction lst act))
+omega_CAction (CSPCommAction (ChanComm c []) a)
+  = (CSPCommAction (ChanComm c []) (omega_CAction a))
 
-omega_CAction lst (CSPRepParalNS (CSExpr cs) [Choose (x,[]) (ZSetDisplay lsx)]
-          (NSExprParam ns [ZVar (x1,[])])
-          (CSPParAction a [ZVar (x2,[])]))
-  = case (x == x1) && (x == x2) of
-    True -> rep_CSPRepParalNS lst omega_CAction a cs ns x lsx
-    _  -> (CSPRepParalNS (CSExpr cs) [Choose (x,[]) (ZSetDisplay lsx)]
-          (NSExprParam ns [ZVar (x1,[])])
-          (omega_CAction lst (CSPParAction a [ZVar (x2,[])])))
-omega_CAction lst (CSPRepParalNS (CSExpr cs) [Choose (x,[]) (ZSetDisplay lsx)]
-          (NSExprParam ns [ZVar (x1,[])]) act)
-  = (CSPRepParalNS (CSExpr cs) [Choose (x,[]) (ZSetDisplay lsx)]
-          (NSExprParam ns [ZVar (x1,[])])
-          (omega_CAction lst act))
-omega_CAction lst (CSPRepInterlNS [Choose (x,[]) (ZSetDisplay lsx)]
-          (NSExprParam ns [ZVar (x1,[])])
-          (CSPParAction a [ZVar (x2,[])]))
-  = case (x == x1) && (x == x2) of
-    True -> rep_CSPRepInterlNS lst omega_CAction a ns x lsx
-    _  ->  (CSPRepInterlNS [Choose (x,[]) (ZSetDisplay lsx)]
-          (NSExprParam ns [ZVar (x1,[])])
-          (omega_CAction lst (CSPParAction a [ZVar (x2,[])])))
-omega_CAction lst (CSPRepInterlNS [Choose (x,[]) (ZSetDisplay lsx)]
-          (NSExprParam ns [ZVar (x1,[])])
-          act)
-  = (CSPRepInterlNS [Choose (x,[]) (ZSetDisplay lsx)]
-          (NSExprParam ns [ZVar (x1,[])])
-          (omega_CAction lst act))
+omega_CAction (CSPCommAction (ChanComm c ((ChanDotExp e):xs)) a)
+  = make_get_com lxs (rename_vars_CAction (CSPCommAction (ChanComm c ((ChanDotExp e):xs)) (omega_prime_CAction a)))
+  where lxs = concat (map get_ZVar_st (free_var_ZExpr e))
 
-omega_CAction lst (CActionCommand (CIf (CircGAction g a)))
-  = make_get_com lst lsx (rename_vars_CAction (map fst lsx) (CActionCommand
-             (CIf (CircGAction g (omega_prime_CAction lst a)))))
-  where
-   lsx = free_var_ZPred g
-omega_CAction lst (CSPCommAction (ChanComm c [ChanInpPred x p]) a)
-  = case not (member x (getWrtV a)) of
-    True -> make_get_com lst lsx (rename_vars_CAction (map fst lsx) (CSPCommAction
+omega_CAction (CSPCommAction (ChanComm c ((ChanOutExp e):xs)) a)
+  = omega_CAction (CSPCommAction (ChanComm c ((ChanDotExp e):xs)) a)
+
+omega_CAction (CSPGuard g a)
+  = make_get_com lxs (rename_vars_CAction (CSPGuard (rename_ZPred g) (omega_prime_CAction a)))
+  where lxs = concat (map get_ZVar_st (free_var_ZPred g))
+
+omega_CAction (CSPCommAction (ChanComm c [ChanInpPred x p]) a)
+  = case not (member x (getWrtV(a))) of
+    True -> make_get_com lsx (rename_vars_CAction (CSPCommAction
              (ChanComm c [ChanInpPred x p])
-                 (omega_prime_CAction lst a)))
+                 (omega_prime_CAction a)))
     _  -> (CSPCommAction (ChanComm c [ChanInpPred x p]) a)
-  where lsx = free_var_ZPred(p)
+  where lsx = concat (map get_ZVar_st (free_var_ZPred p))
 
-omega_CAction lst (CSPCommAction (ChanComm c ((ChanDotExp e):xs)) a)
-  = make_get_com lst lxs (rename_vars_CAction (map fst lxs) (CSPCommAction (ChanComm c ((ChanDotExp e):xs)) (omega_prime_CAction lst a)))
-  where lxs = (get_chan_param ((ChanDotExp e):xs)) `intersect` (filter_state_comp lst)
+omega_CAction (CSPSeq ca cb)
+  = (CSPSeq (omega_CAction ca) (omega_CAction cb))
 
-omega_CAction lst (CActionCommand (CAssign varls valls))
-  = make_get_com lst varls (rename_vars_CAction (map fst (filter_state_comp lst)) (make_set_com lst omega_CAction varls valls CSPSkip))
+omega_CAction (CSPIntChoice ca cb)
+  = (CSPIntChoice (omega_CAction ca) (omega_CAction cb))
 
+omega_CAction (CSPExtChoice ca cb)
+  = make_get_com lsx (rename_vars_CAction (CSPExtChoice (omega_prime_CAction ca) (omega_prime_CAction cb)))
+   where
+    lsx = (map fst (remdups (free_var_CAction (CSPExtChoice ca cb))))
 
-omega_CAction lst (CActionCommand (CIf (CircThenElse gl glx)))
-  = make_get_com lst lsx (rename_vars_CAction (map fst lsx) (CActionCommand (CIf (mk_guard_pair lst omega_prime_CAction guard_pair))))
+omega_CAction (CSPNSParal ns1 cs ns2 a1 a2)
+  = make_get_com lsx (rename_vars_CAction (CSPHide
+   (CSPNSParal NSExpEmpty (CSExpr "MEMi") NSExpEmpty
+     (CSPNSParal NSExpEmpty cs NSExpEmpty
+      (CSPHide
+       (CSPNSParal NSExpEmpty (CSExpr "MEMi") NSExpEmpty
+        (CSPSeq a1 (CSPCommAction (ChanComm "terminate" []) CSPSkip))
+        (CSPParAction "MemoryMerge"
+         [ZSetDisplay [],
+                ZVar ("LEFT",[])]))
+       (CSExpr "MEMi"))
+      (CSPHide
+       (CSPNSParal NSExpEmpty (CSExpr "MEMi") NSExpEmpty
+        (CSPSeq a2 (CSPCommAction (ChanComm "terminate" []) CSPSkip))
+        (CSPParAction "MemoryMerge"
+         [ZSetDisplay [],
+                ZVar ("RIGHT",[])]))
+       (CSExpr "MEMi")))
+      (CActionName "Merge"))
+      (CChanSet ["mleft","mright"])))
+   where
+    lsx = (map fst (remdups  (free_var_CAction a1))) `union` (map fst (remdups  (free_var_CAction a2)))
+
+omega_CAction (CActionCommand (CAssign varls valls))
+  = make_get_com (map fst varls) (rename_vars_CAction (make_set_com omega_CAction varls valls CSPSkip))
+
+omega_CAction (CActionCommand (CIf (CircGAction g a)))
+  = make_get_com lsx (rename_vars_CAction  (CActionCommand
+             (CIf (CircGAction g (omega_prime_CAction a)))))
+  where
+   lsx = (map fst (remdups  (free_var_ZPred g)))
+
+omega_CAction (CActionCommand (CIf (CircThenElse gl glx)))
+  = make_get_com lsx (rename_vars_CAction (CActionCommand (CIf (mk_guard_pair omega_prime_CAction guard_pair))))
   where
    guard_pair = get_guard_pair (CircThenElse gl glx)
-   lsx = concat (map free_var_ZPred (map fst guard_pair))
+   lsx = map fst (remdups $ concat $ map free_var_ZPred (map fst guard_pair))
 
-omega_CAction lst (CSPExtChoice ca cb)
-  = make_get_com lst lsx (rename_vars_CAction (map fst lsx) (CSPExtChoice (omega_prime_CAction lst ca) (omega_prime_CAction lst cb)))
-   where
-    lsx = remdups ((free_var_CAction (CSPExtChoice ca cb)) `intersect` (filter_state_comp lst))
-omega_CAction lst (CSPGuard g a) 
-  = make_get_com lst lxs (rename_vars_CAction (map fst lxs) (CSPGuard (rename_ZPred (map fst lxs) g) (omega_prime_CAction lst a))) 
-    where lxs = remdups (free_var_ZPred(g) `intersect` (filter_state_comp lst))
+omega_CAction (CSPHide a cs) = (CSPHide (omega_CAction a) cs)
+
+omega_CAction (CSPRecursion x c) = (CSPRecursion x (omega_CAction c))
+
+omega_CAction (CActionCommand (CommandBrace g))
+  = omega_CAction (CActionCommand (CPrefix g (ZTrue {reason = []})))
+
+omega_CAction (CActionCommand (CommandBracket g))
+  = omega_CAction (CActionCommand (CPrefix1 g))
+
+omega_CAction (CSPRenAction a (CRenameAssign left right))
+  = (CSPRenAction a (CRename right left))
+
+omega_CAction (CSPRepSeq [Choose (x,[]) v] act)
+  = (CSPRepSeq [Choose (x,[]) v] (omega_CAction act))
+omega_CAction (CSPRepExtChoice [Choose (x,[]) v] act)
+  = (CSPRepExtChoice [Choose (x,[]) v] (omega_CAction act))
+omega_CAction (CSPRepIntChoice [Choose (x,[]) v] act)
+  = (CSPRepIntChoice [Choose (x,[]) v] (omega_CAction act))
+omega_CAction (CSPRepParalNS (CSExpr cs) [Choose (x,[]) (ZSetDisplay lsx)]
+          (NSExprParam ns [ZVar (x1,[])]) act)
+  = (CSPRepParalNS (CSExpr cs) [Choose (x,[]) (ZSetDisplay lsx)]
+          (NSExprParam ns [ZVar (x1,[])]) (omega_CAction act))
+omega_CAction (CSPRepInterlNS [Choose (x,[]) (ZSetDisplay lsx)]
+          (NSExprParam ns [ZVar (x1,[])]) act)
+  = (CSPRepInterlNS [Choose (x,[]) (ZSetDisplay lsx)]
+          (NSExprParam ns [ZVar (x1,[])]) (omega_CAction act))
+-- From now on, I'll be restricting the ZSetDisplay lsx set to ZVar and ZInt - Hope it help me with Isabelle
+omega_CAction (CSPRepSeq [Choose (x,[]) (ZSeqDisplay xs)] (CSPParAction act [ZVar (x1,[])]))
+  = case x == x1 && (is_Var_or_Int xs) of
+    True -> omega_CAction (rep_CSPRepSeq act xs)
+    _  -> (CSPRepSeq [Choose (x,[]) (ZSeqDisplay xs)]
+          (CSPParAction act [ZVar (x1,[])]))
+
+omega_CAction (CSPRepExtChoice [Choose (x,[]) (ZSeqDisplay xs)] (CSPParAction act [ZVar (x1,[])]))
+  = case x == x1 && (is_Var_or_Int xs) of
+    True -> omega_CAction (rep_CSPRepExtChoice act xs)
+    _  -> (CSPRepExtChoice [Choose (x,[]) (ZSeqDisplay xs)]
+          (CSPParAction act [ZVar (x1,[])]))
+
+omega_CAction (CSPRepIntChoice [Choose (x,[]) (ZSeqDisplay xs)]
+          (CSPParAction act [ZVar (x1,[])]))
+  = case x == x1 && (is_Var_or_Int xs) of
+    True -> omega_CAction(rep_CSPRepIntChoice act xs)
+    _  -> (CSPRepIntChoice [Choose (x,[]) (ZSeqDisplay xs)]
+          (CSPParAction act [ZVar (x1,[])]))
+
+omega_CAction (CSPRepParalNS (CSExpr cs) [Choose (x,[]) (ZSetDisplay lsx)]
+          (NSExprParam ns [ZVar (x1,[])])
+          (CSPParAction a [ZVar (x2,[])]))
+  = case (x == x1) && (x == x2) && (is_Var_or_Int lsx) of
+    True -> omega_CAction (rep_CSPRepParalNS a cs ns x lsx)
+    _  -> (CSPRepParalNS (CSExpr cs) [Choose (x,[]) (ZSetDisplay lsx)]
+          (NSExprParam ns [ZVar (x1,[])])
+          (CSPParAction a [ZVar (x2,[])]))
+omega_CAction (CSPRepInterlNS [Choose (x,[]) (ZSetDisplay lsx)]
+          (NSExprParam ns [ZVar (x1,[])])
+          (CSPParAction a [ZVar (x2,[])]))
+  = case (x == x1) && (x == x2) && (is_Var_or_Int lsx) of
+    True -> omega_CAction (rep_CSPRepInterlNS a ns x lsx)
+    _  ->  (CSPRepInterlNS [Choose (x,[]) (ZSetDisplay lsx)]
+          (NSExprParam ns [ZVar (x1,[])])
+          (CSPParAction a [ZVar (x2,[])]))
+omega_CAction x = x
 
 -- Omega Prime
+omega_prime_CAction :: CAction -> CAction
 
-omega_prime_CAction :: [(ZName, ZVar, ZExpr)] -> CAction -> CAction
-omega_prime_CAction lst CSPSkip = CSPSkip
-omega_prime_CAction lst CSPChaos = CSPChaos
-omega_prime_CAction lst CSPStop = CSPStop
-omega_prime_CAction lst (CActionCommand (CAssign varls valls)) = (make_set_com lst omega_CAction varls valls CSPSkip)
-omega_prime_CAction lst (CActionCommand (CIf (CircGAction g a))) = (CActionCommand (CIf (CircGAction g (omega_prime_CAction lst a))))
-omega_prime_CAction lst (CActionCommand (CommandBrace g)) = omega_prime_CAction lst (CActionCommand (CPrefix g (ZTrue {reason = []})))
-omega_prime_CAction lst (CActionCommand (CommandBracket g)) = omega_prime_CAction lst (CActionCommand (CPrefix1 g))
-omega_prime_CAction lst (CActionName n) = (CActionName n)
-omega_prime_CAction lst (CSPCommAction (ChanComm c []) a) = (CSPCommAction (ChanComm c []) (omega_prime_CAction lst a))
-omega_prime_CAction lst (CSPCommAction (ChanComm c x) a) = (CSPCommAction (ChanComm c x) (omega_prime_CAction lst a))
-omega_prime_CAction lst (CSPGuard g a) = (CSPGuard g (omega_prime_CAction lst a))
-omega_prime_CAction lst (CSPHide a cs) = (CSPHide (omega_prime_CAction lst a) cs)
-omega_prime_CAction lst (CSPIntChoice ca cb) = (CSPIntChoice (omega_prime_CAction lst ca) (omega_prime_CAction lst cb))
-omega_prime_CAction lst (CSPRecursion x c) = (CSPRecursion x (omega_prime_CAction lst c))
-omega_prime_CAction lst (CSPRenAction a (CRenameAssign left right)) = (CSPRenAction a (CRename right left))
-omega_prime_CAction lst (CSPSeq ca cb) = (CSPSeq (omega_prime_CAction lst ca) (omega_prime_CAction lst cb))
+omega_prime_CAction (CSPCommAction (ChanComm c []) a)
+  = (CSPCommAction (ChanComm c []) (omega_prime_CAction a))
 
-omega_prime_CAction lst (CActionCommand (CIf (CircThenElse gl glx)))
-  = (CActionCommand (CIf (mk_guard_pair lst omega_prime_CAction guard_pair)))
-  where
-   guard_pair = get_guard_pair (CircThenElse gl glx)
+omega_prime_CAction (CSPCommAction (ChanComm c [ChanDotExp e]) a)
+  = (CSPCommAction (ChanComm c [ChanDotExp (rename_ZExpr e)]) (omega_prime_CAction a))
 
-omega_prime_CAction lst (CSPRepInterlNS [Choose (x,[]) (ZSetDisplay lsx)]
-          (NSExprParam ns [ZVar (x1,[])])
-          (CSPParAction a [ZVar (x2,[])]))
-  = case (x == x1) && (x == x2) of
-    True -> rep_CSPRepInterlNS lst omega_prime_CAction a ns x lsx
-    _  ->  (CSPRepInterlNS [Choose (x,[]) (ZSetDisplay lsx)]
-          (NSExprParam ns [ZVar (x1,[])])
-          (omega_prime_CAction lst (CSPParAction a [ZVar (x2,[])])))
-omega_prime_CAction lst (CSPRepInterlNS [Choose (x,[]) (ZSetDisplay lsx)]
-          (NSExprParam ns [ZVar (x1,[])])
-          act)
-  = (CSPRepInterlNS [Choose (x,[]) (ZSetDisplay lsx)]
-          (NSExprParam ns [ZVar (x1,[])])
-          (omega_prime_CAction lst act))
+omega_prime_CAction (CSPSeq ca cb)
+  = (CSPSeq (omega_prime_CAction ca) (omega_CAction cb))
 
-omega_prime_CAction lst (CSPRepParalNS (CSExpr cs) [Choose (x,[]) (ZSetDisplay lsx)]
-          (NSExprParam ns [ZVar (x1,[])])
-          (CSPParAction a [ZVar (x2,[])]))
-  = case (x == x1) && (x == x2) of
-    True -> rep_CSPRepParalNS lst omega_prime_CAction a cs ns x lsx
-    _  -> (CSPRepParalNS (CSExpr cs) [Choose (x,[]) (ZSetDisplay lsx)]
-          (NSExprParam ns [ZVar (x1,[])])
-          (omega_prime_CAction lst (CSPParAction a [ZVar (x2,[])])))
-omega_prime_CAction lst (CSPRepParalNS (CSExpr cs) [Choose (x,[]) (ZSetDisplay lsx)]
-          (NSExprParam ns [ZVar (x1,[])]) act)
-  = (CSPRepParalNS (CSExpr cs) [Choose (x,[]) (ZSetDisplay lsx)]
-          (NSExprParam ns [ZVar (x1,[])])
-          (omega_prime_CAction lst act))
+omega_prime_CAction x = omega_CAction x
 
-omega_prime_CAction lst (CSPRepSeq [Choose (x,[]) (ZSeqDisplay xs)] (CSPParAction act [ZVar (x1,[])]))
-  = case x == x1 of
-    True -> omega_prime_CAction lst (rep_CSPRepSeq lst omega_prime_CAction act xs)
-    _  -> (CSPRepSeq [Choose (x,[]) (ZSeqDisplay xs)]
-          (omega_prime_CAction lst (CSPParAction act [ZVar (x1,[])])))
-omega_prime_CAction lst (CSPRepSeq [Choose (x,[]) v] act) = (CSPRepSeq [Choose (x,[]) v] (omega_prime_CAction lst act))
-omega_prime_CAction lst (CSPRepExtChoice [Choose (x,[]) (ZSeqDisplay xs)] (CSPParAction act [ZVar (x1,[])]))
-  = case x == x1 of
-    True -> rep_CSPRepExtChoice lst omega_prime_CAction act xs
-    _  -> (CSPRepExtChoice [Choose (x,[]) (ZSeqDisplay xs)]
-          (CSPParAction act [ZVar (x1,[])]))
-
-omega_prime_CAction lst (CSPRepIntChoice [Choose (x,[]) (ZSeqDisplay xs)]
-          (CSPParAction act [ZVar (x1,[])]))
-  = case x == x1 of
-    True -> rep_CSPRepIntChoice lst omega_prime_CAction act xs
-    _  -> (CSPRepIntChoice [Choose (x,[]) (ZSeqDisplay xs)]
-          (CSPParAction act [ZVar (x1,[])]))
-omega_prime_CAction lst (CSPRepIntChoice [Choose (x,[]) v] act) = (CSPRepIntChoice [Choose (x,[]) v] (omega_prime_CAction lst act))
-
-
-free_var_CAction :: CAction -> [ZVar]
-free_var_CAction (CActionCommand c) = (free_var_comnd c)
-free_var_CAction (CSPCommAction (ChanComm com xs) c) = (get_chan_param xs)++(free_var_CAction c)
-free_var_CAction (CSPGuard p c) = (free_var_ZPred p)++(free_var_CAction c)
-free_var_CAction (CSPSeq ca cb) = (free_var_CAction ca)++(free_var_CAction cb)
-free_var_CAction (CSPExtChoice ca cb) = (free_var_CAction ca)++(free_var_CAction cb)
-free_var_CAction (CSPIntChoice ca cb) = (free_var_CAction ca)++(free_var_CAction cb)
-free_var_CAction (CSPNSParal ns1 cs ns2 ca cb) = (free_var_CAction ca)++(free_var_CAction cb)
-free_var_CAction (CSPParal cs ca cb) = (free_var_CAction ca)++(free_var_CAction cb)
-free_var_CAction (CSPNSInter ns1 ns2 ca cb) = (free_var_CAction ca)++(free_var_CAction cb)
-free_var_CAction (CSPInterleave ca cb) = (free_var_CAction ca)++(free_var_CAction cb)
-free_var_CAction (CSPHide c cs) = (free_var_CAction c)
-free_var_CAction (CSPRecursion nm c) = (free_var_CAction c)
-free_var_CAction (CSPUnParAction lst c nm) =setminus (free_var_CAction c) (fvs free_var_ZGenFilt lst)
-free_var_CAction (CSPRepSeq lst c) = setminus (free_var_CAction c) (fvs free_var_ZGenFilt lst)
-free_var_CAction (CSPRepExtChoice lst c) = setminus(free_var_CAction c) (fvs free_var_ZGenFilt lst)
-free_var_CAction (CSPRepIntChoice lst c) = setminus(free_var_CAction c) (fvs free_var_ZGenFilt lst)
-free_var_CAction (CSPRepParalNS cs lst ns c) = setminus (free_var_CAction c) (fvs free_var_ZGenFilt lst)
-free_var_CAction (CSPRepParal cs lst c) = setminus (free_var_CAction c) (fvs free_var_ZGenFilt lst)
-free_var_CAction (CSPRepInterlNS lst ns c) = setminus (free_var_CAction c) (fvs free_var_ZGenFilt lst)
-free_var_CAction (CSPRepInterl lst c) = setminus (free_var_CAction c) (fvs free_var_ZGenFilt lst)
-free_var_CAction _ = []
-
-
-free_var_comnd :: CCommand -> [ZVar]
-free_var_comnd (CAssign v e) = v
-free_var_comnd (CIf ga) = free_var_if ga
-free_var_comnd (CVarDecl z c) = setminus (free_var_CAction c) (fvs free_var_ZGenFilt z)
-free_var_comnd (CommandBrace z) = (free_var_ZPred z)
-free_var_comnd (CommandBracket z) = (free_var_ZPred z)
-free_var_comnd (CValDecl z c) = setminus (free_var_CAction c) (fvs free_var_ZGenFilt z)
-free_var_comnd (CResDecl z c) = setminus (free_var_CAction c) (fvs free_var_ZGenFilt z)
-free_var_comnd (CVResDecl z c) = setminus (free_var_CAction c) (fvs free_var_ZGenFilt z)
-free_var_comnd _ = []
-
-free_var_if :: CGActions -> [ZVar]
-free_var_if (CircGAction p a) = (free_var_ZPred p)++(free_var_CAction a)
-free_var_if (CircThenElse ga gb) = (free_var_if ga)++(free_var_if gb)
-free_var_if (CircElse (CircusAction a)) = (free_var_CAction a)
-free_var_if (CircElse (ParamActionDecl x (CircusAction a))) = setminus (free_var_CAction a) (fvs free_var_ZGenFilt x)
