test_haskabelle/OmegaDefs.hs
@@ -1,60 +1,87 @@
 module OmegaDefs
-(
-filter_state_comp,
-free_var_ZExpr,
-free_var_ZGenFilt,
-free_var_ZPred,
-fvs,
-get_chan_param,
-get_guard_pair,
-get_proc_name,
-intersect,
-make_get_com,
-member,
-mk_guard_pair, rename_ZPred,
-remdups,
-rename_vars_CAction,
-rep_CSPRepExtChoice, 
-rep_CSPRepIntChoice, 
-rep_CSPRepInterlNS, 
-rep_CSPRepParalNS, 
-rep_CSPRepSeq, 
-setminus,
-union,
-make_set_com, getWrtV)
 where
 import AST
-filter_state_comp :: [(ZName, ZVar, ZExpr)] -> [ZVar]
-filter_state_comp [] = []
-filter_state_comp [(_, v, _)] = [v]
-filter_state_comp ((_, v, _):xs) = [v]++(filter_state_comp xs)
 
 
-get_guard_pair :: CGActions -> [(ZPred, CAction)]
-get_guard_pair (CircThenElse (CircGAction g2 a2) (CircGAction g3 a3)) = [(g2,a2),(g3,a3)]
-get_guard_pair (CircThenElse (CircGAction g1 a1) glx) = [(g1,a1)]++(get_guard_pair glx)
-get_guard_pair _ = []
+join_name n v = n ++ "_" ++ v
 
 
-get_proc_name :: ZName -> [(ZName, ZVar, ZExpr)] -> ZName
-get_proc_name x [(a,(va,x1),b)]
- = case x == va of
-  True -> a
-  _ -> ""
-get_proc_name x ((a,(va,x1),b):vst)
- = case x == va of
-  True -> a
-  _ -> get_proc_name x vst
+free_var_CAction :: CAction -> [ZVar]
+free_var_CAction (CActionCommand c)
+ = (free_var_comnd c)
+free_var_CAction (CSPCommAction (ChanComm com xs) c)
+ = (get_chan_var xs)++(free_var_CAction c)
+free_var_CAction (CSPGuard p c)
+ = (free_var_ZPred p)++(free_var_CAction c)
+free_var_CAction (CSPSeq ca cb)
+ = (free_var_CAction ca)++(free_var_CAction cb)
+free_var_CAction (CSPExtChoice ca cb)
+ = (free_var_CAction ca)++(free_var_CAction cb)
+free_var_CAction (CSPIntChoice ca cb)
+ = (free_var_CAction ca)++(free_var_CAction cb)
+free_var_CAction (CSPNSParal ns1 cs ns2 ca cb)
+ = (free_var_CAction ca)++(free_var_CAction cb)
+free_var_CAction (CSPParal cs ca cb)
+ = (free_var_CAction ca)++(free_var_CAction cb)
+free_var_CAction (CSPNSInter ns1 ns2 ca cb)
+ = (free_var_CAction ca)++(free_var_CAction cb)
+free_var_CAction (CSPInterleave ca cb)
+ = (free_var_CAction ca)++(free_var_CAction cb)
+free_var_CAction (CSPHide c cs)
+ = (free_var_CAction c)
+free_var_CAction (CSPRecursion nm c)
+ = (free_var_CAction c)
+free_var_CAction (CSPUnParAction lst c nm)
+ =  (setminus (free_var_CAction c) (fvs free_var_ZGenFilt lst))
+free_var_CAction (CSPRepSeq lst c)
+ =  (setminus (free_var_CAction c) (fvs free_var_ZGenFilt lst))
+free_var_CAction (CSPRepExtChoice lst c)
+ =  (setminus (free_var_CAction c) (fvs free_var_ZGenFilt lst))
+free_var_CAction (CSPRepIntChoice lst c)
+ =  (setminus (free_var_CAction c) (fvs free_var_ZGenFilt lst))
+free_var_CAction (CSPRepParalNS cs lst ns c)
+ =  (setminus (free_var_CAction c) (fvs free_var_ZGenFilt lst))
+free_var_CAction (CSPRepParal cs lst c)
+ =  (setminus (free_var_CAction c) (fvs free_var_ZGenFilt lst))
+free_var_CAction (CSPRepInterlNS lst ns c)
+ =  (setminus (free_var_CAction c) (fvs free_var_ZGenFilt lst))
+free_var_CAction (CSPRepInterl lst c)
+ =  (setminus (free_var_CAction c) (fvs free_var_ZGenFilt lst))
+free_var_CAction _ = []
 
+free_var_comnd (CAssign v e)
+ = v
+free_var_comnd (CIf ga)
+ = free_var_if ga
+free_var_comnd (CVarDecl z c)
+ =  (setminus (free_var_CAction c) (fvs free_var_ZGenFilt z))
+free_var_comnd (CAssumpt n p1 p2)
+ = []
+free_var_comnd (CAssumpt1 n p)
+ = []
+free_var_comnd (CPrefix p1 p2)
+ = []
+free_var_comnd (CPrefix1 p)
+ = []
+free_var_comnd (CommandBrace z)
+ = (free_var_ZPred z)
+free_var_comnd (CommandBracket z)
+ = (free_var_ZPred z)
+free_var_comnd (CValDecl z c)
+ =  (setminus (free_var_CAction c) (fvs free_var_ZGenFilt z))
+free_var_comnd (CResDecl z c)
+ =  (setminus (free_var_CAction c) (fvs free_var_ZGenFilt z))
+free_var_comnd (CVResDecl z c)
+ =  (setminus (free_var_CAction c) (fvs free_var_ZGenFilt z))
 
-make_get_com :: [(ZName, ZVar, ZExpr)] -> [ZVar] -> CAction -> CAction
-make_get_com lst [(x,[])] c = (CSPCommAction (ChanComm "mget"[ChanDotExp (ZVar ((get_proc_name x lst)++"_"++x,[])),ChanInp ("v"++(get_proc_name x lst)++"_"++x)]) c)
-make_get_com lst ((x,[]):xs) c = (CSPCommAction (ChanComm "mget"[ChanDotExp (ZVar ((get_proc_name x lst)++"_"++x,[])),ChanInp ("v"++(get_proc_name x lst)++"_"++x)]) (make_get_com lst xs c))
-make_get_com lst x c = c
-
--- All that should be found in the Defsets.hs file
-getWrtV :: t -> [t1]
-getWrtV xs = []
+free_var_if (CircGAction p a)
+ = (free_var_ZPred p)++(free_var_CAction a)
+free_var_if (CircThenElse ga gb)
+ = (free_var_if ga)++(free_var_if gb)
+free_var_if (CircElse (CircusAction a))
+ = (free_var_CAction a)
+free_var_if (CircElse (ParamActionDecl x (CircusAction a)))
+ =  (setminus (free_var_CAction a) (fvs free_var_ZGenFilt x))
 
 free_var_ZGenFilt :: ZGenFilt -> [ZVar]
 free_var_ZGenFilt (Choose v e) = [v]
@@ -68,7 +95,7 @@ free_var_ZPred (ZTrue{reason=p})
   = error "Don't know what free vars of ZTrue are right now. Check back later"
 free_var_ZPred (ZAnd a b)
  = free_var_ZPred a ++ free_var_ZPred b
-
+free_var_ZPred x = error "Don't know what free vars of this right now. Check back later"
 
 fvs :: (t -> [t1]) -> [t] -> [t1]
 fvs f [] = []
@@ -85,18 +112,122 @@ free_var_ZExpr(ZCall ex ex2) = free_var_ZExpr ex2 -- is this right??
 free_var_ZExpr _ = []
 
 
-rename_vars_CReplace :: t -> CReplace -> CReplace
-rename_vars_CReplace lst (CRename zvarls1 zvarls) = (CRename zvarls1 zvarls)
-rename_vars_CReplace lst (CRenameAssign zvarls1 zvarls) = (CRenameAssign zvarls1 zvarls)
+
+get_chan_var :: [CParameter] -> [ZVar]
+get_chan_var [] = []
+get_chan_var [ChanDotExp (ZVar (x,_))]
+ = [(x,[])]
+get_chan_var [ChanOutExp (ZVar (x,_))]
+ = [(x,[])]
+get_chan_var [_]
+ = []
+get_chan_var ((ChanDotExp (ZVar (x,_))):xs)
+ = [(x,[])]++(get_chan_var xs)
+get_chan_var ((ChanOutExp (ZVar (x,_))):xs)
+ = [(x,[])]++(get_chan_var xs)
+get_chan_var (_:xs) = (get_chan_var xs)
 
 
-rename_ZPred :: [String] -> ZPred -> ZPred
-rename_ZPred lst (ZFalse{reason=a}) = (ZFalse{reason=a})
-rename_ZPred lst (ZTrue{reason=a}) = (ZTrue{reason=a})
-rename_ZPred lst (ZAnd p1 p2) = (ZAnd (rename_ZPred lst p1) (rename_ZPred lst p2))
+get_guard_pair :: CGActions -> [(ZPred, CAction)]
+get_guard_pair (CircThenElse (CircGAction g2 a2) (CircGAction g3 a3)) = [(g2,a2),(g3,a3)]
+get_guard_pair (CircThenElse (CircGAction g1 a1) glx) = [(g1,a1)]++(get_guard_pair glx)
+get_guard_pair _ = []
 
 
-inListVar :: Eq a => a -> [a] -> Bool
+make_get_com :: [ZName] -> CAction -> CAction
+make_get_com [x] c = (CSPCommAction (ChanComm "mget"[ChanDotExp (ZVar (x,[])),ChanInp ("v_"++x)]) c)
+make_get_com (x:xs) c = (CSPCommAction (ChanComm "mget"[ChanDotExp (ZVar (x,[])),ChanInp ("v_"++x)]) (make_get_com xs c))
+make_get_com x c = c    
+
+make_set_com f [(x,_)] [y] c = (CSPCommAction (ChanComm "mset"[ChanDotExp (ZVar (x,[])),ChanOutExp y]) (f c))
+make_set_com f ((x,_):xs) (y:ys) c = (CSPCommAction (ChanComm "mset"[ChanDotExp (ZVar (x,[])),ChanOutExp y]) (make_set_com f xs ys c))
+
+
+mk_guard_pair f [(g,a)] = (CircGAction g (f a))
+mk_guard_pair f ((g,a):ls) = (CircThenElse (CircGAction g (f a)) (mk_guard_pair f ls))
+
+-- All that should be found in the Defsets.hs file
+getWrtV :: t -> [t1]
+getWrtV xs = []
+
+
+
+rename_vars_CAction :: CAction -> CAction
+rename_vars_CAction (CActionCommand cmd) = (CActionCommand (rename_vars_CCommand cmd))
+rename_vars_CAction (CActionName zn) = (CActionName zn)
+rename_vars_CAction (CSPSkip ) = (CSPSkip )
+rename_vars_CAction (CSPStop ) = (CSPStop )
+rename_vars_CAction (CSPChaos) = (CSPChaos)
+rename_vars_CAction (CSPCommAction c a) = (CSPCommAction (rename_vars_Comm c) (rename_vars_CAction a))
+rename_vars_CAction (CSPGuard zp a) = (CSPGuard (rename_ZPred zp) (rename_vars_CAction a))
+rename_vars_CAction (CSPSeq a1 a2) = (CSPSeq (rename_vars_CAction a1) (rename_vars_CAction a2))
+rename_vars_CAction (CSPExtChoice a1 a2) = (CSPExtChoice (rename_vars_CAction a1) (rename_vars_CAction a2))
+rename_vars_CAction (CSPIntChoice a1 a2) = (CSPIntChoice (rename_vars_CAction a1) (rename_vars_CAction a2))
+rename_vars_CAction (CSPNSParal ns1 cs ns2 a1 a2) = (CSPNSParal ns1 cs ns2 (rename_vars_CAction a1) (rename_vars_CAction a2))
+rename_vars_CAction (CSPParal cs a1 a2) = (CSPParal cs (rename_vars_CAction a1) (rename_vars_CAction a2))
+rename_vars_CAction (CSPNSInter ns1 ns2 a1 a2) = (CSPNSInter ns1 ns2 (rename_vars_CAction a1) (rename_vars_CAction a2))
+rename_vars_CAction (CSPInterleave a1 a2) = (CSPInterleave (rename_vars_CAction a1) (rename_vars_CAction a2))
+rename_vars_CAction (CSPHide a cs) = (CSPHide (rename_vars_CAction a) cs)
+rename_vars_CAction (CSPParAction zn zexprls) = (CSPParAction zn (map (rename_ZExpr) zexprls))
+rename_vars_CAction (CSPRenAction zn crpl) = (CSPRenAction zn crpl)
+rename_vars_CAction (CSPRecursion zn a) = (CSPRecursion zn (rename_vars_CAction a))
+rename_vars_CAction (CSPUnParAction zgf a zn) = (CSPUnParAction zgf (rename_vars_CAction a) zn)
+rename_vars_CAction (CSPRepSeq zgf a) = (CSPRepSeq zgf (rename_vars_CAction a))
+rename_vars_CAction (CSPRepExtChoice zgf a) = (CSPRepExtChoice zgf (rename_vars_CAction a))
+rename_vars_CAction (CSPRepIntChoice zgf a) = (CSPRepIntChoice zgf (rename_vars_CAction a))
+rename_vars_CAction (CSPRepParalNS cs zgf ns a) = (CSPRepParalNS cs zgf ns (rename_vars_CAction a))
+rename_vars_CAction (CSPRepParal cs zgf a) = (CSPRepParal cs zgf (rename_vars_CAction a))
+rename_vars_CAction (CSPRepInterlNS zgf ns a) = (CSPRepInterlNS zgf ns (rename_vars_CAction a))
+rename_vars_CAction (CSPRepInterl zgf a) = (CSPRepInterl zgf (rename_vars_CAction a))
+
+rename_vars_CCommand :: CCommand -> CCommand
+rename_vars_CCommand (CAssign zvarls1 zexprls) = (CAssign (map rename_vars_Zvar zvarls1) (map (rename_ZExpr) zexprls))
+rename_vars_CCommand (CIf ga) = (CIf (rename_vars_CGActions ga))
+rename_vars_CCommand (CVarDecl zgf a) = (CVarDecl zgf (rename_vars_CAction a))
+rename_vars_CCommand (CAssumpt znls zp1 zp2) = (CAssumpt znls (rename_ZPred zp1) zp2)
+rename_vars_CCommand (CAssumpt1 znls zp) = (CAssumpt1 znls zp)
+rename_vars_CCommand (CPrefix zp1 zp2) = (CPrefix (rename_ZPred zp1) zp2)
+rename_vars_CCommand (CPrefix1 zp) = (CPrefix1 zp)
+rename_vars_CCommand (CommandBrace zp) = (CommandBrace zp)
+rename_vars_CCommand (CommandBracket zp) = (CommandBracket zp)
+rename_vars_CCommand (CValDecl zgf a) = (CValDecl zgf (rename_vars_CAction a))
+rename_vars_CCommand (CResDecl zgf a) = (CResDecl zgf (rename_vars_CAction a))
+rename_vars_CCommand (CVResDecl zgf a) = (CVResDecl zgf (rename_vars_CAction a))
+
+rename_vars_Comm :: Comm -> Comm
+rename_vars_Comm (ChanComm zn cpls) = (ChanComm zn (map (rename_vars_CParameter) cpls))
+rename_vars_Comm (ChanGenComm zn zexprls cpls) = (ChanGenComm zn (map (rename_ZExpr) zexprls) (map (rename_vars_CParameter) cpls))
+
+rename_vars_CParameter :: CParameter -> CParameter
+rename_vars_CParameter (ChanInp zn) = (ChanInp zn)
+rename_vars_CParameter (ChanInpPred zn zp) = (ChanInpPred zn (rename_ZPred zp))
+rename_vars_CParameter (ChanOutExp ze) = (ChanOutExp (rename_ZExpr ze))
+rename_vars_CParameter (ChanDotExp ze) = (ChanDotExp (rename_ZExpr ze))
+
+rename_vars_CGActions :: CGActions -> CGActions
+rename_vars_CGActions (CircGAction zp a) = (CircGAction (rename_ZPred zp) (rename_vars_CAction a))
+rename_vars_CGActions (CircThenElse cga1 cga2) = (CircThenElse (rename_vars_CGActions cga1) (rename_vars_CGActions cga2))
+rename_vars_CGActions (CircElse pa) = (CircElse pa)
+
+rename_ZPred :: ZPred -> ZPred
+rename_ZPred (ZFalse{reason=a}) = (ZFalse{reason=a})
+rename_ZPred (ZTrue{reason=a}) = (ZTrue{reason=a})
+rename_ZPred (ZAnd p1 p2) = (ZAnd (rename_ZPred p1) (rename_ZPred p2))
+
+rename_ZExpr :: ZExpr -> ZExpr
+rename_ZExpr (ZVar (va,x))
+  = case (is_ZVar_st va) of
+        True -> (ZVar ("v_"++va,x))
+        False -> (ZVar (va,x))
+rename_ZExpr (ZInt zi) = (ZInt zi)
+rename_ZExpr (ZCall xpr1 xpr2) = (ZCall (rename_ZExpr xpr1) (rename_ZExpr xpr2))
+
+
+rename_vars_CReplace :: CReplace -> CReplace
+rename_vars_CReplace (CRename zvarls1 zvarls) = (CRename zvarls1 zvarls)
+rename_vars_CReplace (CRenameAssign zvarls1 zvarls) = (CRenameAssign zvarls1 zvarls)
+
+inListVar :: a -> [a] -> Bool
 inListVar x []
  = False
 inListVar x [va]
@@ -108,141 +239,71 @@ inListVar x (va:vst)
   True -> True
   _ -> inListVar x vst
 
+bindingsVar :: [(ZVar, ZExpr)] -> [(ZVar, ZExpr)]
+bindingsVar [] = []
+bindingsVar [((va,x),b)]
+  = case (is_ZVar_st va) of
+          True -> [(("v_"++va,x),(rename_ZExpr b))]
+          False -> [((va,x),(rename_ZExpr b))]
+bindingsVar (((va,x),b):xs)
+  = case (is_ZVar_st va) of
+          True -> [(("v_"++va,x),(rename_ZExpr b))]++(bindingsVar xs)
+          False -> [((va,x),(rename_ZExpr b))]++(bindingsVar xs)
 
-rename_ZExpr :: [String] -> ZExpr -> ZExpr
-rename_ZExpr lst (ZVar (va,x))
-  = case (inListVar va lst) of
-        True -> (ZVar ("v_"++va,x))
-        False -> (ZVar (va,x))
-rename_ZExpr lst (ZInt zi) = (ZInt zi)
-rename_ZExpr lst (ZCall xpr1 xpr2) = (ZCall (rename_ZExpr lst xpr1) (rename_ZExpr lst xpr2))
+rename_vars_Zvar (a,x)
+ = case (isPrefixOf "st_var_" a) of
+    True -> ((join_name "v" a),x)
+    _ -> (a,x)
+get_ZVar_st (a,x)
+ = case (isPrefixOf "st_var_" a) of
+    True -> [a]
+    _ -> []
+is_ZVar_st a = isPrefixOf "st_var_" a
 
-
-bindingsVar :: [String] -> [(ZVar, ZExpr)] -> [(ZVar, ZExpr)]
-bindingsVar lst []
-  = []
-bindingsVar lst [((va,x),b)]
-  = case (inListVar va lst) of
-          True -> [(("v_"++va,x),(rename_ZExpr lst b))]
-          False -> [((va,x),(rename_ZExpr lst b))]
-bindingsVar lst (((va,x),b):xs)
-  = case (inListVar va lst) of
-          True -> [(("v_"++va,x),(rename_ZExpr lst b))]++(bindingsVar lst xs)
-          False -> [((va,x),(rename_ZExpr lst b))]++(bindingsVar lst xs)
-
-
-
-rename_vars_CAction :: [String] -> CAction -> CAction
-rename_vars_CAction lst (CActionCommand cmd) = (CActionCommand (rename_vars_CCommand lst cmd))
-rename_vars_CAction lst (CActionName zn) = (CActionName zn)
-rename_vars_CAction lst (CSPSkip ) = (CSPSkip )
-rename_vars_CAction lst (CSPStop ) = (CSPStop )
-rename_vars_CAction lst (CSPChaos) = (CSPChaos)
-rename_vars_CAction lst (CSPCommAction c a) = (CSPCommAction (rename_vars_Comm lst c) (rename_vars_CAction lst a))
-rename_vars_CAction lst (CSPGuard zp a) = (CSPGuard (rename_ZPred lst zp) (rename_vars_CAction lst a))
-rename_vars_CAction lst (CSPSeq a1 a2) = (CSPSeq (rename_vars_CAction lst a1) (rename_vars_CAction lst a2))
-rename_vars_CAction lst (CSPExtChoice a1 a2) = (CSPExtChoice (rename_vars_CAction lst a1) (rename_vars_CAction lst a2))
-rename_vars_CAction lst (CSPIntChoice a1 a2) = (CSPIntChoice (rename_vars_CAction lst a1) (rename_vars_CAction lst a2))
-rename_vars_CAction lst (CSPNSParal ns1 cs ns2 a1 a2) = (CSPNSParal ns1 cs ns2 (rename_vars_CAction lst a1) (rename_vars_CAction lst a2))
-rename_vars_CAction lst (CSPParal cs a1 a2) = (CSPParal cs (rename_vars_CAction lst a1) (rename_vars_CAction lst a2))
-rename_vars_CAction lst (CSPNSInter ns1 ns2 a1 a2) = (CSPNSInter ns1 ns2 (rename_vars_CAction lst a1) (rename_vars_CAction lst a2))
-rename_vars_CAction lst (CSPInterleave a1 a2) = (CSPInterleave (rename_vars_CAction lst a1) (rename_vars_CAction lst a2))
-rename_vars_CAction lst (CSPHide a cs) = (CSPHide (rename_vars_CAction lst a) cs)
-rename_vars_CAction lst (CSPParAction zn zexprls) = (CSPParAction zn (map (rename_ZExpr lst) zexprls))
-rename_vars_CAction lst (CSPRenAction zn crpl) = (CSPRenAction zn (rename_vars_CReplace lst crpl))
-rename_vars_CAction lst (CSPRecursion zn a) = (CSPRecursion zn (rename_vars_CAction lst a))
-rename_vars_CAction lst (CSPUnParAction zgf a zn) = (CSPUnParAction zgf (rename_vars_CAction lst a) zn)
-rename_vars_CAction lst (CSPRepSeq zgf a) = (CSPRepSeq zgf (rename_vars_CAction lst a))
-rename_vars_CAction lst (CSPRepExtChoice zgf a) = (CSPRepExtChoice zgf (rename_vars_CAction lst a))
-rename_vars_CAction lst (CSPRepIntChoice zgf a) = (CSPRepIntChoice zgf (rename_vars_CAction lst a))
-rename_vars_CAction lst (CSPRepParalNS cs zgf ns a) = (CSPRepParalNS cs zgf ns (rename_vars_CAction lst a))
-rename_vars_CAction lst (CSPRepParal cs zgf a) = (CSPRepParal cs zgf (rename_vars_CAction lst a))
-rename_vars_CAction lst (CSPRepInterlNS zgf ns a) = (CSPRepInterlNS zgf ns (rename_vars_CAction lst a))
-rename_vars_CAction lst (CSPRepInterl zgf a) = (CSPRepInterl zgf (rename_vars_CAction lst a))
-
-rename_vars_CCommand :: [String] -> CCommand -> CCommand
-rename_vars_CCommand lst (CAssign zvarls1 zexprls) = (CAssign zvarls1 (map (rename_ZExpr lst) zexprls))
-rename_vars_CCommand lst (CIf ga) = (CIf (rename_vars_CGActions lst ga))
-rename_vars_CCommand lst (CVarDecl zgf a) = (CVarDecl zgf (rename_vars_CAction lst a))
-rename_vars_CCommand lst (CAssumpt znls zp1 zp2) = (CAssumpt znls (rename_ZPred lst zp1) zp2)
-rename_vars_CCommand lst (CAssumpt1 znls zp) = (CAssumpt1 znls zp)
-rename_vars_CCommand lst (CPrefix zp1 zp2) = (CPrefix (rename_ZPred lst zp1) zp2)
-rename_vars_CCommand lst (CPrefix1 zp) = (CPrefix1 zp)
-rename_vars_CCommand lst (CommandBrace zp) = (CommandBrace zp)
-rename_vars_CCommand lst (CommandBracket zp) = (CommandBracket zp)
-rename_vars_CCommand lst (CValDecl zgf a) = (CValDecl zgf (rename_vars_CAction lst a))
-rename_vars_CCommand lst (CResDecl zgf a) = (CResDecl zgf (rename_vars_CAction lst a))
-rename_vars_CCommand lst (CVResDecl zgf a) = (CVResDecl zgf (rename_vars_CAction lst a))
-
-rename_vars_Comm :: [String] -> Comm -> Comm
-rename_vars_Comm lst (ChanComm zn cpls) = (ChanComm zn (map (rename_vars_CParameter lst) cpls))
-rename_vars_Comm lst (ChanGenComm zn zexprls cpls) = (ChanGenComm zn (map (rename_ZExpr lst) zexprls) (map (rename_vars_CParameter lst) cpls))
-
-rename_vars_CParameter :: [String] -> CParameter -> CParameter
-rename_vars_CParameter lst (ChanInp zn) = (ChanInp zn)
-rename_vars_CParameter lst (ChanInpPred zn zp) = (ChanInpPred zn (rename_ZPred lst zp))
-rename_vars_CParameter lst (ChanOutExp ze) = (ChanOutExp (rename_ZExpr lst ze))
-rename_vars_CParameter lst (ChanDotExp ze) = (ChanDotExp (rename_ZExpr lst ze))
-
-rename_vars_CGActions :: [String] -> CGActions -> CGActions
-rename_vars_CGActions lst (CircGAction zp a) = (CircGAction (rename_ZPred lst zp) (rename_vars_CAction lst a))
-rename_vars_CGActions lst (CircThenElse cga1 cga2) = (CircThenElse (rename_vars_CGActions lst cga1) (rename_vars_CGActions lst cga2))
-rename_vars_CGActions lst (CircElse pa) = (CircElse pa)
+is_Var_or_Int [ZVar (a,b)] = True
+is_Var_or_Int [ZInt x] = True
+is_Var_or_Int ((ZVar (a,b)):xs) = True && is_Var_or_Int xs
+is_Var_or_Int ((ZInt x):xs) = True && is_Var_or_Int xs
+is_Var_or_Int _ = False
 
 
-get_chan_param :: [CParameter] -> [ZVar]
-get_chan_param [] = []
-get_chan_param [ChanDotExp (ZVar (x,_))] = [(x,[])]
-get_chan_param [ChanOutExp (ZVar (x,_))] = [(x,[])]
-get_chan_param [_] = []
-get_chan_param ((ChanDotExp (ZVar (x,_))):xs) = [(x,[])]++(get_chan_param xs)
-get_chan_param ((ChanOutExp (ZVar (x,_))):xs) = [(x,[])]++(get_chan_param xs)
-get_chan_param (_:xs) = (get_chan_param xs)
+rep_CSPRepSeq :: ZName -> [ZExpr] -> CAction
+rep_CSPRepSeq a [x]
+  = (CSPParAction a [x])
+rep_CSPRepSeq a (x:xs)
+  = CSPSeq (CSPParAction a [x]) (rep_CSPRepSeq a xs)
 
+rep_CSPRepIntChoice :: ZName -> [ZExpr] -> CAction
+rep_CSPRepIntChoice a [x]
+  = (CSPParAction a [x])
+rep_CSPRepIntChoice a (x:xs)
+  = CSPIntChoice (CSPParAction a [x]) (rep_CSPRepIntChoice a xs)
 
+rep_CSPRepExtChoice :: ZName -> [ZExpr] -> CAction
+rep_CSPRepExtChoice a [x]
+  = (CSPParAction a [x])
+rep_CSPRepExtChoice a (x:xs)
+  = CSPExtChoice (CSPParAction a [x]) (rep_CSPRepExtChoice a xs)
 
--- Extra from MappingFunStatelesssCircus.lhs
-rep_CSPRepSeq lst f a [x]
-  = f lst (CSPParAction a [x])
-rep_CSPRepSeq lst f a (x:xs)
-  = CSPSeq (f lst (CSPParAction a [x])) (rep_CSPRepSeq lst f a xs)
-
-rep_CSPRepIntChoice lst f a [x]
-  = f lst (CSPParAction a [x])
-rep_CSPRepIntChoice lst f a (x:xs)
-  = CSPIntChoice (f lst (CSPParAction a [x])) (rep_CSPRepIntChoice lst f a xs)
-
-rep_CSPRepExtChoice lst f a [x]
-  =  f lst (CSPParAction a [x])
-rep_CSPRepExtChoice lst f a (x:xs)
-  = CSPExtChoice ( f lst (CSPParAction a [x])) (rep_CSPRepExtChoice lst f a xs)
-
-rep_CSPRepParalNS lst f a _ _ _ [x]
-  =  f lst (CSPParAction a [x])
-rep_CSPRepParalNS lst f a cs ns y (x:xs)
+rep_CSPRepParalNS :: ZName -> ZName -> ZName -> String -> [ZExpr] -> CAction
+rep_CSPRepParalNS a _ _ _ [x]
+  = (CSPParAction a [x])
+rep_CSPRepParalNS a cs ns y (x:xs)
   = (CSPNSParal (NSExprParam ns [x]) (CSExpr cs)
     (NSBigUnion (ZSetComp
            [Choose (y,[]) (ZSetDisplay xs)]
            (Just (ZCall (ZVar (ns,[])) (ZVar (y,[])))) ) )
-     ( f lst (CSPParAction a [x])) (rep_CSPRepParalNS lst f a cs ns y xs) )
+     (CSPParAction a [x]) (rep_CSPRepParalNS a cs ns y xs) )
 
-rep_CSPRepInterlNS lst f a _ _ [x]
-  =  f lst (CSPParAction a [x])
-rep_CSPRepInterlNS lst f a ns y (x:xs)
+rep_CSPRepInterlNS :: ZName -> ZName -> String -> [ZExpr] -> CAction
+rep_CSPRepInterlNS a _ _ [x]
+  = (CSPParAction a [x])
+rep_CSPRepInterlNS a ns y (x:xs)
   = (CSPNSInter (NSExprParam ns [x])
     (NSBigUnion (ZSetComp
            [Choose (y,[]) (ZSetDisplay xs)]
            (Just (ZCall (ZVar (ns,[])) (ZVar (y,[])))) ) )
-     ( f lst (CSPParAction a [x])) (rep_CSPRepInterlNS lst f a ns y xs) )
-
---
-
-mk_guard_pair lst f [(g,a)] = (CircGAction g (f lst a))
-mk_guard_pair lst f ((g,a):ls) = (CircThenElse (CircGAction g (f lst a)) (mk_guard_pair lst f ls))
-
-
-make_set_com lst f [(x,[])] [y] c = (CSPCommAction (ChanComm "mset"[ChanDotExp (ZVar ((get_proc_name x lst)++"_"++x,[])),ChanOutExp y]) (f lst c))
-make_set_com lst f (((x,[])):xs) (y:ys) c = (CSPCommAction (ChanComm "mset"[ChanDotExp (ZVar ((get_proc_name x lst)++"_"++x,[])),ChanOutExp y]) (make_set_com lst f xs ys c))
+     (CSPParAction a [x]) (rep_CSPRepInterlNS a ns y xs) )
 
 
  -- Artur - 15/12/2016
@@ -277,27 +338,11 @@ intersect (a:x) y = if member a y then a : (intersect x y) else intersect x y
 union [] y = y
 union (a:x) y = if (member a y) then (union x y) else a : (union x y);
 
-remdups :: (Eq a) => [a] -> [a]
+remdups :: [a] -> [a]
 remdups [] = []
 remdups (x:xs)
  | member x xs  = remdups xs
  | otherwise = x : remdups xs
--- | 'delete' @x@ removes the first occurrence of @x@ from its list argument.
--- For example,
---
--- > delete 'a' "banana" == "bnana"
---
--- It is a special case of 'deleteBy', which allows the programmer to
--- supply their own equality test.
-
-delete                  :: (Eq a) => a -> [a] -> [a]
-delete                  =  deleteBy (==)
-
--- | The 'deleteBy' function behaves like 'delete', but takes a
--- user-supplied equality predicate.
-deleteBy                :: (a -> a -> Bool) -> a -> [a] -> [a]
-deleteBy _  _ []        = []
-deleteBy eq x (y:ys)    = if x `eq` y then ys else y : deleteBy eq x ys
 
 
 -- Not exported:
@@ -310,3 +355,10 @@ elem_by _  _ []         =  False
 elem_by eq y (x:xs)     =  y `eq` x || elem_by eq y xs
 
 
+
+-- | The 'isPrefixOf' function takes two lists and returns 'True'
+-- iff the first list is a prefix of the second.
+isPrefixOf              :: [a] -> [a] -> Bool
+isPrefixOf [] _         =  True
+isPrefixOf _  []        =  False
+isPrefixOf (x:xs) (y:ys)=  x == y && isPrefixOf xs ys
