test_haskabelle/haskabelle/MappingFunStatelessCircus.thy
@@ -2,119 +2,58 @@ theory MappingFunStatelessCircus
 imports AST OmegaDefs Prelude
 begin
  
-function (sequential) omega_CAction :: "(ZName * ZVar * ZExpr) list \<Rightarrow> CAction \<Rightarrow> CAction" and 
-    omega_prime_CAction :: "(ZName * ZVar * ZExpr) list \<Rightarrow> CAction \<Rightarrow> CAction"
+function (sequential) omega_CAction :: "CAction \<Rightarrow> CAction" and 
+    omega_prime_CAction :: "CAction \<Rightarrow> CAction"
 where
-  "omega_CAction lst CSPSkip = CSPSkip"
-| "omega_CAction lst CSPStop = CSPStop"
-| "omega_CAction lst CSPChaos = CSPChaos"
-| "omega_CAction lst (CSPCommAction (ChanComm c ((ChanOutExp e) # xs)) a) = omega_CAction lst (CSPCommAction (ChanComm c ((ChanDotExp e) # xs)) a)"
-| "omega_CAction lst (CSPSeq ca cb) = (CSPSeq (omega_CAction lst ca) (omega_CAction lst cb))"
-| "omega_CAction lst (CSPIntChoice ca cb) = (CSPIntChoice (omega_CAction lst ca) (omega_CAction lst cb))"
-| "omega_CAction lst (CSPCommAction (ChanComm c Nil) a) = (CSPCommAction (ChanComm c Nil) (omega_CAction lst a))"
-| "omega_CAction lst (CSPHide a cs) = (CSPHide (omega_CAction lst a) cs)"
-| "omega_CAction lst (CSPRecursion x c) = (CSPRecursion x (omega_CAction lst c))"
-| "omega_CAction lst (CActionCommand (CommandBrace g)) = omega_CAction lst (CActionCommand (CPrefix g (ZTrue Nil)))"
-| "omega_CAction lst (CActionCommand (CommandBracket g)) = omega_CAction lst (CActionCommand (CPrefix1 g))"
-| "omega_CAction lst (CSPRenAction a (CRenameAssign left right)) = (CSPRenAction a (CRename right left))"
-(*| "omega_CAction lst (CSPRepSeq [Choose (x, Nil) (ZSeqDisplay xs)] (CSPParAction act [ZVar (x1, Nil)])) 
-    = (case x = x1 of 
-        True \<Rightarrow> omega_CAction lst (rep_CSPRepSeq lst omega_CAction act xs) 
-        | _ \<Rightarrow> (CSPRepSeq [Choose (x, Nil) (ZSeqDisplay xs)] (omega_CAction lst (CSPParAction act [ZVar (x1, Nil)]))))"
-| "omega_CAction lst (CSPRepExtChoice [Choose (x, Nil) (ZSeqDisplay xs)] (CSPParAction act [ZVar (x1, Nil)])) 
-    = (case x = x1 of 
-        True \<Rightarrow> rep_CSPRepExtChoice lst omega_CAction act xs 
-        | _ \<Rightarrow> (CSPRepExtChoice [Choose (x, Nil) (ZSeqDisplay xs)] (CSPParAction act [ZVar (x1, Nil)])))"
-| "omega_CAction lst (CSPRepIntChoice [Choose (x, Nil) (ZSeqDisplay xs)] (CSPParAction act [ZVar (x1, Nil)])) 
-    = (case x = x1 of 
-        True \<Rightarrow> rep_CSPRepIntChoice lst omega_CAction act xs 
-        | _ \<Rightarrow> (CSPRepIntChoice [Choose (x, Nil) (ZSeqDisplay xs)] (CSPParAction act [ZVar (x1, Nil)])))"
-| "omega_CAction lst (CSPRepParalNS (CSExpr cs) [Choose (x, Nil) (ZSetDisplay lsx)] (NSExprParam ns [ZVar (x1, Nil)]) (CSPParAction a [ZVar (x2, Nil)])) 
-    = (case (x = x1) & (x = x2) of 
-        True \<Rightarrow> rep_CSPRepParalNS lst omega_CAction a cs ns x lsx 
-        | _ \<Rightarrow> (CSPRepParalNS (CSExpr cs) [Choose (x, Nil) (ZSetDisplay lsx)] (NSExprParam ns [ZVar (x1, Nil)]) (omega_CAction lst (CSPParAction a [ZVar (x2, Nil)]))))"
-| "omega_CAction lst (CSPRepInterlNS [Choose (x, Nil) (ZSetDisplay lsx)] (NSExprParam ns [ZVar (x1, Nil)]) (CSPParAction a [ZVar (x2, Nil)])) 
-    = (case (x = x1) & (x = x2) of 
-        True \<Rightarrow> rep_CSPRepInterlNS lst omega_CAction a ns x lsx 
-        | _ \<Rightarrow> (CSPRepInterlNS [Choose (x, Nil) (ZSetDisplay lsx)] (NSExprParam ns [ZVar (x1, Nil)]) (omega_CAction lst (CSPParAction a [ZVar (x2, Nil)]))))"
-| "omega_CAction lst (CActionCommand (CIf (CircGAction g a))) 
-    = (let lsx = free_var_ZPred g 
-        in make_get_com lst lsx (rename_vars_CAction (map fst lsx) (CActionCommand (CIf (CircGAction g (omega_prime_CAction lst a))))))"
-*)(* | "omega_CAction lst (CSPRepInterlNS [Choose (x, Nil) (ZSetDisplay lsx)] (NSExprParam ns [ZVar (x1, Nil)]) act)
-    = (CSPRepInterlNS [Choose (x, Nil) (ZSetDisplay lsx)] (NSExprParam ns [ZVar (x1, Nil)]) (omega_CAction lst act))"*)
-(* | "omega_CAction lst (CSPRepParalNS (CSExpr cs) [Choose (x, Nil) (ZSetDisplay lsx)] (NSExprParam ns [ZVar (x1, Nil)]) act) 
-    = (CSPRepParalNS (CSExpr cs) [Choose (x, Nil) (ZSetDisplay lsx)] (NSExprParam ns [ZVar (x1, Nil)]) (omega_CAction lst act))"*)
-(* | "omega_CAction lst (CSPRepIntChoice [Choose (x, Nil) v] act) = (CSPRepIntChoice [Choose (x, Nil) v] (omega_CAction lst act))"*)
-(* | "omega_CAction lst (CSPRepExtChoice [Choose (x, Nil) v] act) = (CSPRepExtChoice [Choose (x, Nil) v] (omega_CAction lst act))"*)
-(* | "omega_CAction lst (CSPRepSeq [Choose (x, Nil) v] act) = (CSPRepSeq [Choose (x, Nil) v] (omega_CAction lst act))"*)   
-| "omega_CAction lst (CSPCommAction (ChanComm c [ChanInpPred x p]) a) 
-    = (let lsx = free_var_ZPred p 
-        in case Not (member x (getWrtV a)) of 
-            True \<Rightarrow> make_get_com lst lsx (rename_vars_CAction (map fst lsx) (CSPCommAction (ChanComm c [ChanInpPred x p]) (omega_prime_CAction lst a))) 
-            | _ \<Rightarrow> (CSPCommAction (ChanComm c [ChanInpPred x p]) a))"
-| "omega_CAction lst (CActionCommand (CAssign varls valls)) 
-    = make_get_com lst varls (rename_vars_CAction (map fst (filter_state_comp lst)) (make_set_com lst omega_CAction varls valls CSPSkip))"
-| "omega_CAction lst (CActionCommand (CIf (CircThenElse gl glx))) 
-    = (let guard_pair = get_guard_pair (CircThenElse gl glx); 
-           lsx = concat (map free_var_ZPred (map fst guard_pair)) 
-      in make_get_com lst lsx (rename_vars_CAction (map fst lsx) (CActionCommand (CIf (mk_guard_pair lst omega_prime_CAction guard_pair)))))"
-| "omega_CAction lst (CSPCommAction (ChanComm c ((ChanDotExp e) # xs)) a) 
-    = (let lxs = intersect (get_chan_param ((ChanDotExp e) # xs)) (filter_state_comp lst) 
-       in make_get_com lst lxs (rename_vars_CAction (map fst lxs) (CSPCommAction (ChanComm c ((ChanDotExp e) # xs)) (omega_prime_CAction lst a))))"
-| "omega_CAction lst (CSPExtChoice ca cb) 
-    = (let lsx = remdups (intersect (free_var_CAction (CSPExtChoice ca cb)) (filter_state_comp lst)) 
-      in make_get_com lst lsx (rename_vars_CAction (map fst lsx) (CSPExtChoice (omega_prime_CAction lst ca) (omega_prime_CAction lst cb))))"
-| "omega_CAction lst (CSPGuard g a) 
-    = (let lxs = remdups (intersect (free_var_ZPred g) (filter_state_comp lst)) 
-      in make_get_com lst lxs (rename_vars_CAction (map fst lxs) (CSPGuard (rename_ZPred (map fst lxs) g) (omega_prime_CAction lst a))))"
-| "omega_CAction lst x = x"
-| "omega_prime_CAction lst CSPSkip = CSPSkip"
-| "omega_prime_CAction lst CSPChaos = CSPChaos"
-| "omega_prime_CAction lst CSPStop = CSPStop"
-| "omega_prime_CAction lst (CActionCommand (CAssign varls valls)) = (make_set_com lst omega_CAction varls valls CSPSkip)"
-| "omega_prime_CAction lst (CActionCommand (CIf (CircGAction g a))) = (CActionCommand (CIf (CircGAction g (omega_prime_CAction lst a))))"
-| "omega_prime_CAction lst (CActionCommand (CommandBrace g)) = omega_prime_CAction lst (CActionCommand (CPrefix g (ZTrue Nil)))"
-| "omega_prime_CAction lst (CActionCommand (CommandBracket g)) = omega_prime_CAction lst (CActionCommand (CPrefix1 g))"
-| "omega_prime_CAction lst (CActionName n) = (CActionName n)"
-| "omega_prime_CAction lst (CSPCommAction (ChanComm c Nil) a) = (CSPCommAction (ChanComm c Nil) (omega_prime_CAction lst a))"
-| "omega_prime_CAction lst (CSPCommAction (ChanComm c x) a) = (CSPCommAction (ChanComm c x) (omega_prime_CAction lst a))"
-| "omega_prime_CAction lst (CSPGuard g a) = (CSPGuard g (omega_prime_CAction lst a))"
-| "omega_prime_CAction lst (CSPHide a cs) = (CSPHide (omega_prime_CAction lst a) cs)"
-| "omega_prime_CAction lst (CSPIntChoice ca cb) = (CSPIntChoice (omega_prime_CAction lst ca) (omega_prime_CAction lst cb))"
-| "omega_prime_CAction lst (CSPRecursion x c) = (CSPRecursion x (omega_prime_CAction lst c))"
-| "omega_prime_CAction lst (CSPRenAction a (CRenameAssign left right)) = (CSPRenAction a (CRename right left))"
-| "omega_prime_CAction lst (CSPSeq ca cb) = (CSPSeq (omega_prime_CAction lst ca) (omega_prime_CAction lst cb))"
-| "omega_prime_CAction lst (CActionCommand (CIf (CircThenElse gl glx))) = (let guard_pair = get_guard_pair (CircThenElse gl glx) in (CActionCommand (CIf (mk_guard_pair lst omega_prime_CAction guard_pair))))"
-(*| "omega_prime_CAction lst (CSPRepInterlNS [Choose (x, Nil) (ZSetDisplay lsx)] (NSExprParam ns [ZVar (x1, Nil)]) (CSPParAction a [ZVar (x2, Nil)])) 
-    = (case (x = x1) & (x = x2) of 
-        True \<Rightarrow> rep_CSPRepInterlNS lst omega_prime_CAction a ns x lsx 
-        | _ \<Rightarrow> (CSPRepInterlNS [Choose (x, Nil) (ZSetDisplay lsx)] (NSExprParam ns [ZVar (x1, Nil)]) (omega_prime_CAction lst (CSPParAction a [ZVar (x2, Nil)]))))"
-| "omega_prime_CAction lst (CSPRepInterlNS [Choose (x, Nil) (ZSetDisplay lsx)] (NSExprParam ns [ZVar (x1, Nil)]) act) 
-    = (CSPRepInterlNS [Choose (x, Nil) (ZSetDisplay lsx)] (NSExprParam ns [ZVar (x1, Nil)]) (omega_prime_CAction lst act))"
-| "omega_prime_CAction lst (CSPRepParalNS (CSExpr cs) [Choose (x, Nil) (ZSetDisplay lsx)] (NSExprParam ns [ZVar (x1, Nil)]) (CSPParAction a [ZVar (x2, Nil)])) 
-    = (case (x = x1) & (x = x2) of 
-        True \<Rightarrow> rep_CSPRepParalNS lst omega_prime_CAction a cs ns x lsx 
-        | _ \<Rightarrow> (CSPRepParalNS (CSExpr cs) [Choose (x, Nil) (ZSetDisplay lsx)] (NSExprParam ns [ZVar (x1, Nil)]) (omega_prime_CAction lst (CSPParAction a [ZVar (x2, Nil)]))))"
-| "omega_prime_CAction lst (CSPRepParalNS (CSExpr cs) [Choose (x, Nil) (ZSetDisplay lsx)] (NSExprParam ns [ZVar (x1, Nil)]) act) 
-    = (CSPRepParalNS (CSExpr cs) [Choose (x, Nil) (ZSetDisplay lsx)] (NSExprParam ns [ZVar (x1, Nil)]) (omega_prime_CAction lst act))"
-| "omega_prime_CAction lst (CSPRepSeq [Choose (x, Nil) (ZSeqDisplay xs)] (CSPParAction act [ZVar (x1, Nil)])) 
-    = (case x = x1 of 
-        True \<Rightarrow> omega_prime_CAction lst (rep_CSPRepSeq lst omega_prime_CAction act xs) 
-        | _ \<Rightarrow> (CSPRepSeq [Choose (x, Nil) (ZSeqDisplay xs)] (omega_prime_CAction lst (CSPParAction act [ZVar (x1, Nil)]))))"
-| "omega_prime_CAction lst (CSPRepSeq [Choose (x, Nil) v] act) 
-    = (CSPRepSeq [Choose (x, Nil) v] (omega_prime_CAction lst act))"
-| "omega_prime_CAction lst (CSPRepExtChoice [Choose (x, Nil) (ZSeqDisplay xs)] (CSPParAction act [ZVar (x1, Nil)])) 
-    = (case x = x1 of 
-        True \<Rightarrow> rep_CSPRepExtChoice lst omega_prime_CAction act xs 
-        | _ \<Rightarrow> (CSPRepExtChoice [Choose (x, Nil) (ZSeqDisplay xs)] (CSPParAction act [ZVar (x1, Nil)])))"
-| "omega_prime_CAction lst (CSPRepIntChoice [Choose (x, Nil) (ZSeqDisplay xs)] (CSPParAction act [ZVar (x1, Nil)])) 
-    = (case x = x1 of 
-        True \<Rightarrow> rep_CSPRepIntChoice lst omega_prime_CAction act xs 
-        | _ \<Rightarrow> (CSPRepIntChoice [Choose (x, Nil) (ZSeqDisplay xs)] (CSPParAction act [ZVar (x1, Nil)])))"
-| "omega_prime_CAction lst (CSPRepIntChoice [Choose (x, Nil) v] act) 
-    = (CSPRepIntChoice [Choose (x, Nil) v] (omega_prime_CAction lst act))"
-*)
-| "omega_prime_CAction lst x = x"
-  by pat_completeness auto
-    
+  "omega_CAction CSPSkip = CSPSkip"
+| "omega_CAction CSPStop = CSPStop"
+| "omega_CAction CSPChaos = CSPChaos"
+| "omega_CAction (CSPCommAction (ChanComm c Nil) a) = (CSPCommAction (ChanComm c Nil) (omega_CAction a))"
+| "omega_CAction (CSPCommAction (ChanComm c ((ChanDotExp e) # xs)) a) = (let lxs = concat (map get_ZVar_st (free_var_ZExpr e))
+                                                                         in make_get_com lxs (rename_vars_CAction (CSPCommAction (ChanComm c ((ChanDotExp e) # xs)) (omega_prime_CAction a))))"
+| "omega_CAction (CSPCommAction (ChanComm c ((ChanOutExp e) # xs)) a) = omega_CAction (CSPCommAction (ChanComm c ((ChanDotExp e) # xs)) a)"
+| "omega_CAction (CSPGuard g a) = (let lxs = concat (map get_ZVar_st (free_var_ZPred g))
+                                   in make_get_com lxs (rename_vars_CAction (CSPGuard (rename_ZPred g) (omega_prime_CAction a))))"
+| "omega_CAction (CSPCommAction (ChanComm c [ChanInpPred x p]) a) = (let lsx = concat (map get_ZVar_st (free_var_ZPred p))
+                                                                     in case Not (member x (getWrtV a)) of
+                                                                           True \<Rightarrow> make_get_com lsx (rename_vars_CAction (CSPCommAction (ChanComm c [ChanInpPred x p]) (omega_prime_CAction a)))
+                                                                         | _ \<Rightarrow> (CSPCommAction (ChanComm c [ChanInpPred x p]) a))"
+| "omega_CAction (CSPSeq ca cb) = (CSPSeq (omega_CAction ca) (omega_CAction cb))"
+| "omega_CAction (CSPIntChoice ca cb) = (CSPIntChoice (omega_CAction ca) (omega_CAction cb))"
+| "omega_CAction (CSPExtChoice ca cb) = (let lsx = (map fst (remdups (free_var_CAction (CSPExtChoice ca cb))))
+                                         in make_get_com lsx (rename_vars_CAction (CSPExtChoice (omega_prime_CAction ca) (omega_prime_CAction cb))))"
+| "omega_CAction (CSPNSParal ns1 cs ns2 a1 a2) = (let lsx = union (map fst (remdups (free_var_CAction a1))) (map fst (remdups (free_var_CAction a2)))
+                                                  in make_get_com lsx (rename_vars_CAction (CSPHide (CSPNSParal NSExpEmpty (CSExpr ''MEMi'') NSExpEmpty (CSPNSParal NSExpEmpty cs NSExpEmpty (CSPHide (CSPNSParal NSExpEmpty (CSExpr ''MEMi'') NSExpEmpty (CSPSeq a1 (CSPCommAction (ChanComm ''terminate'' Nil) CSPSkip)) (CSPParAction ''MemoryMerge'' [ZSetDisplay Nil, ZVar (''LEFT'', Nil)])) (CSExpr ''MEMi'')) (CSPHide (CSPNSParal NSExpEmpty (CSExpr ''MEMi'') NSExpEmpty (CSPSeq a2 (CSPCommAction (ChanComm ''terminate'' Nil) CSPSkip)) (CSPParAction ''MemoryMerge'' [ZSetDisplay Nil, ZVar (''RIGHT'', Nil)])) (CSExpr ''MEMi''))) (CActionName ''Merge'')) (CChanSet [''mleft'', ''mright'']))))"
+| "omega_CAction (CActionCommand (CAssign varls valls)) = make_get_com (map fst varls) (rename_vars_CAction (make_set_com omega_CAction varls valls CSPSkip))"
+| "omega_CAction (CActionCommand (CIf (CircGAction g a))) = (let lsx = (map fst (remdups (free_var_ZPred g)))
+                                                             in make_get_com lsx (rename_vars_CAction (CActionCommand (CIf (CircGAction g (omega_prime_CAction a))))))"
+| "omega_CAction (CActionCommand (CIf (CircThenElse gl glx))) = (let guard_pair = get_guard_pair (CircThenElse gl glx);
+                                                                     lsx = map fst (remdups $ (concat $ map free_var_ZPred (map fst guard_pair)))
+                                                                 in make_get_com lsx (rename_vars_CAction (CActionCommand (CIf (mk_guard_pair omega_prime_CAction guard_pair)))))"
+| "omega_CAction (CSPHide a cs) = (CSPHide (omega_CAction a) cs)"
+| "omega_CAction (CSPRecursion x c) = (CSPRecursion x (omega_CAction c))"
+| "omega_CAction (CActionCommand (CommandBrace g)) = omega_CAction (CActionCommand (CPrefix g (ZTrue Nil)))"
+| "omega_CAction (CActionCommand (CommandBracket g)) = omega_CAction (CActionCommand (CPrefix1 g))"
+| "omega_CAction (CSPRenAction a (CRenameAssign left right)) = (CSPRenAction a (CRename right left))"
+(*| "omega_CAction (CSPRepSeq [Choose (x, Nil) (ZSeqDisplay xs)] (CSPParAction act [ZVar (x1, Nil)])) = (case (x = x1) & (is_Var_or_Int xs) of True \<Rightarrow> omega_CAction (rep_CSPRepSeq act xs))"
+| "omega_CAction (CSPRepExtChoice [Choose (x, Nil) (ZSeqDisplay xs)] (CSPParAction act [ZVar (x1, Nil)])) = (case x = x1 & (is_Var_or_Int xs) of True \<Rightarrow> omega_CAction (rep_CSPRepExtChoice act xs))"
+| "omega_CAction (CSPRepIntChoice [Choose (x, Nil) (ZSeqDisplay xs)] (CSPParAction act [ZVar (x1, Nil)])) = (case x = x1 & (is_Var_or_Int xs) of True \<Rightarrow> omega_CAction (rep_CSPRepIntChoice act xs))"
+| "omega_CAction (CSPRepParalNS (CSExpr cs) [Choose (x, Nil) (ZSetDisplay lsx)] (NSExprParam ns [ZVar (x1, Nil)]) (CSPParAction a [ZVar (x2, Nil)])) = (case ((x = x1) & (x = x2)) & (is_Var_or_Int lsx) of
+                                                                                                                                                           True \<Rightarrow> omega_CAction (rep_CSPRepParalNS a cs ns x lsx)
+                                                                                                                                                         | _ \<Rightarrow> (CSPRepParalNS (CSExpr cs) [Choose (x, Nil) (ZSetDisplay lsx)] (NSExprParam ns [ZVar (x1, Nil)]) (CSPParAction a [ZVar (x2, Nil)])))"
+| "omega_CAction (CSPRepInterlNS [Choose (x, Nil) (ZSetDisplay lsx)] (NSExprParam ns [ZVar (x1, Nil)]) (CSPParAction a [ZVar (x2, Nil)])) = (case ((x = x1) & (x = x2)) & (is_Var_or_Int lsx) of
+                                                                                                                                                True \<Rightarrow> omega_CAction (rep_CSPRepInterlNS a ns x lsx)
+                                                                                                                                              | _ \<Rightarrow> (CSPRepInterlNS [Choose (x, Nil) (ZSetDisplay lsx)] (NSExprParam ns [ZVar (x1, Nil)]) (CSPParAction a [ZVar (x2, Nil)])))"
+*)| "omega_CAction (CSPRepSeq [Choose (x, Nil) v] act) = (CSPRepSeq [Choose (x, Nil) v] (omega_CAction act))"
+| "omega_CAction (CSPRepExtChoice [Choose (x, Nil) v] act) = (CSPRepExtChoice [Choose (x, Nil) v] (omega_CAction act))"
+| "omega_CAction (CSPRepIntChoice [Choose (x, Nil) v] act) = (CSPRepIntChoice [Choose (x, Nil) v] (omega_CAction act))"
+| "omega_CAction (CSPRepParalNS (CSExpr cs) [Choose (x, Nil) (ZSetDisplay lsx)] (NSExprParam ns [ZVar (x1, Nil)]) act) = (CSPRepParalNS (CSExpr cs) [Choose (x, Nil) (ZSetDisplay lsx)] (NSExprParam ns [ZVar (x1, Nil)]) (omega_CAction act))"
+| "omega_CAction (CSPRepInterlNS [Choose (x, Nil) (ZSetDisplay lsx)] (NSExprParam ns [ZVar (x1, Nil)]) act) = (CSPRepInterlNS [Choose (x, Nil) (ZSetDisplay lsx)] (NSExprParam ns [ZVar (x1, Nil)]) (omega_CAction act))"
+| "omega_CAction x = x"
+| "omega_prime_CAction (CSPCommAction (ChanComm c Nil) a) = (CSPCommAction (ChanComm c Nil) (omega_prime_CAction a))"
+| "omega_prime_CAction (CSPCommAction (ChanComm c [ChanDotExp e]) a) = (CSPCommAction (ChanComm c [ChanDotExp (rename_ZExpr e)]) (omega_prime_CAction a))"
+| "omega_prime_CAction (CSPSeq ca cb) = (CSPSeq (omega_prime_CAction ca) (omega_CAction cb))"
+| "omega_prime_CAction x = omega_CAction x"
+by pat_completeness auto
+
 end
